<?xml version="1.0" encoding="UTF-8"?>

<section xml:id="sec-2nd-order-linear-const-coeff-repeated" xmlns:xi="http://www.w3.org/2001/XInclude">
  <title>Second-order Linear ODEs with Constant Coefficients - Repeated Real Roots</title>

<subsection xml:id="sec-2nd-order-linear-const-coeff-repeated-1">
  <title>The formula of the general solution</title>
  <p>Consider the ODE
    <me>ay'' + by' + cy = 0</me>
    where <m>a, b, c</m> are constant numbers. We tried the function <m>y = e^{rt}</m> and got the auxiliary equation
    <me>ar^2 + br + c = 0.</me>
    If the quadratic equation has two repeated roots <m>r_1 = r_2 = r,</m> in this case, we only obtain one solution
    <me>y_1 = e^{rt}.</me>
    Another solution may be obtained (via cheating) by
    <me>y_2 = te^{rt}.</me>
    The general solution is
    <me>y = C_1 e^{rt} + C_2 te^{rt}.</me>
 </p>

<example> 
<title><m>y'' - 2y' + y = 0.</m></title> 
<ul>
<li>Auxiliary equation: <m>r^2 - 2r + 1 = 0 \implies r_1 = r_2 = 1.</m></li>
<li>General solution: <m>y = C_1 e^t + C_2 te^t.</m></li>
</ul>
</example>

<example> 
<title><m>4y'' - 4y' + y = 0.</m></title> 
<ul>
<li>Auxiliary equation: <m>4r^2 - 4r + 1 = 0 \implies r_1 = r_2 = \frac{1}{2}.</m></li>
<li>General solution: <m>y = C_1 e^{\frac{t}{2}} + C_2 te^{\frac{t}{2}}.</m></li>
</ul>
</example>

<example>
<title>For the IVP <m>y'' + 10y' + 25y = 0, \, y(0) = 1, \, y'(0) = \alpha,</m>find the critical value of <m>\alpha</m> where the long-term behavior changes.</title> 
<ul>
<li>Auxiliary equation: <m>r^2 + 10r + 25 = 0 \implies r_1 = r_2 = -5.</m></li>
<li>General solution: <m>y = C_1 e^{-5t} + C_2 t e^{-5t}.</m></li>
<li>Plug in the initial values: 
<md>
<mrow>y(0) = 1 \implies C_1 = 1.</mrow>
<mrow>y'(0) = \alpha \implies -5C_1 + C_2 = \alpha \implies C_2 = \alpha + 5.</mrow>
</md>
Solution of the IVP: <me>y = e^{-5t} + (\alpha + 5) t e^{-5t}.</me></li>
<li><p>As <m>t \to \infty,</m> the solution <m>y \to 0</m> no matter how <m>\alpha</m> is chosen. However, there are two ways approaching zero:</p>
<p>If <m>\alpha \gt -5,</m> then <m>y \to 0^+.</m> If <m>\alpha \lt -5,</m> then <m>y \to 0^-.</m></p></li>
</ul>
<p>Conclusuion: The long-term behavior changes when <m>\alpha = -5.</m></p>

<p>
  <!-- Space for figure -->
</p>
<p>
  <strong>For <m>\alpha \gt -5:</m></strong>
  <m>y(t) = (1 + (\alpha + 5)t)e^{-5t}, \, \alpha \gt 0.</m>
</p>

<p>
  <!-- Space for figure -->
</p>
<p>
  <strong>For <m>\alpha \lt -5:</m></strong>
  <m>y(t) = (1 + (\alpha + 5)t)e^{-5t}, \, \alpha \lt 0.</m>
</p>

<p>
  <!-- Space for figure -->
</p>
</example>
</subsection>

<subsection xml:id="sec-2nd-order-linear-const-coeff-repeated-2">
  <title>The method of reduction of order</title>

<p>How do we know we should multiply by <m>t?</m> It is a result of a very standard technique called <term>variation of parameters</term>.</p>

<p><alert>Philosophy:</alert> If you know one solution <m>y_1(t),</m> then since the ODE is linear, for any number <m>c,</m> the function <m>cy_1</m> would also be a solution.</p>
<p><alert>Variation of parameter</alert> simply means that replacing the numerical parameter <m>c</m> with a function <m>u(t),</m> i.e., set
  <me>y_2(t) = u(t)y_1(t).</me>
Plugging it back into the ODE, we may get an (usually much simpler) ODE for <m>u.</m> By solving for <m>u,</m> we may obtain <m>y_2.</m></p>
<p>In the context of linear homogeneous ODE, the technique is usually referred to as <term>reduction of order</term>.</p>


<p>Let <m>y_1</m> be a solution of the homogeneous linear ODE
<me>y'' + p(t)y' + q(t)y = 0.</me>
We set <m>y_2(t) = u(t)y_1(t)</m> and require that <m>y_2</m> is another solution. This means that
<me>(uy_1)'' + p(uy_1)' + quy_1 = 0</me>
Expanding the left-hand-side:
<md>
<mrow>LHS \amp= u''y_1 + 2u'y_1' + uy_1''</mrow>
<mrow>\amp= u''y_1 + (2y_1' + py_1)u' + pu'y_1 + quy_1</mrow>
<mrow>\amp= u''y_1 + (2y_1' + py_1)u' + u(y_1'' + py_1' + qy_1)</mrow>
<mrow>\amp= u''y_1 + (2y_1' + py_1)u' = 0 = RHS</mrow>
</md>
we obtain a second-order ODE of <m>u</m> that involves only <m>u''</m> and <m>u'</m>. </p>

<p>This ODE is essentially a first-order separable ODE of <m>u'</m>, i.e.,
<me>y_1 \frac{du'}{dt} = -(2y_1' + py_1)u' \implies \frac{du'}{u'} = -\frac{2y_1' + py_1}{y_1} dt</me>
Solving <m>u'</m> then integrate, we obtain <m>u</m> and thus <m>y_2.</m></p>

<remark>
<ol>
<li>When formulating the equation for <m>u'</m>, make sure you read the function <m>p</m> from the <alert>standard form</alert>.</li>
<li>Since we only need one <m>y_2</m> that is linearly independent to <m>y_1</m>, when solving for <m>u'</m> and integrating for <m>u</m>, we may make a <alert>wise choice</alert> of the arbitrary constants. It suffices that <m>u' \neq 0.</m></li>
<li>It is possible to have a formula for <m>u</m>, namely,
<me>u(t) = \int \dfrac{\exp(-\int p(t)dt)}{y_1(t)^2} dt</me>
I do not recommend using this formula or memorizing it.</li>
</ol>
</remark>

<example>
<title>How to find the <m>t</m>-factor in the repeated root case</title>
<p>Let <m>ay'' + by' + cy = 0</m> be an ODE whose auxiliary equation has repeated roots <m>r_1 = r_2 = r</m>. This means that the ODE can be rewritten as
<me>y'' - 2ry' + r^2y = 0.</me>
For <m>y_1 = e^{rt}</m>, we set <m>y_2 = uy_1</m>, then
<md>
<mrow>\amp y_2'' - 2ry_2' + r^2y_2 = (y_1)'' - 2r(y_1)' + r^2uy_1</mrow>
<mrow>\amp= u''y_1 + 2u'y_1' + uy_1'' - 2r(u'y_1 + uy_1') + r^2uy_1</mrow>
<mrow>\amp= u''e^{rt} + 2u' \cdot re^{rt} + u \cdot r^2e^{rt} - 2ru'e^{rt} - 2r \cdot re^{rt} + r^2ue^{rt}</mrow>
<mrow>\amp= u''e^{rt} - 2ru'e^{rt} + r^2ue^{rt} = 0</mrow>
<mrow>\amp= e^{rt}u'' = 0 \implies u'' = 0 \implies u' = C_1</mrow>
</md>
For convenience, we pick <m>C_1 = 1</m> so that <m>u' \neq 0</m>, then integrate to get <m>u = t,</m> thus <me>y_2 = te^{rt}.</me> 
The condition that <m>u'\neq 0</m> automatically guarantees that <m>W(y_1, y_2) \neq 0</m> [Why?]. We conclude that <me>y = C_1e^{rt} + C_2te^{rt}</me> is the general solution.</p>
</example>


<example>
<title>For the ODE <m>ty'' - y' - 4t^3y = 0,</m> knowing that <m>y_1 = \sin(t^2)</m> is a solution, find the general solution.</title>
<ul>
<li>Standard form: <me>y'' - \dfrac{1}{t}y' - 4t^2y = 0 \implies p(t) = -\dfrac{1}{t}.</me></li>
<li>Set <m>y_2 = uy_1.</m> To formulate the ODE for <m>u',</m> we have
<me>y_1 = \sin(t^2), \quad y_1' = 2t \cos(t^2)</me>
Plug them into the ODE
<me>y_1u'' + (2y_1' + py_1)u' = 0,</me>
we have
<md>
<mrow> \amp \sin(t^2) \dfrac{du'}{dt} + \left(4t \cos(t^2) - \dfrac{1}{t} \sin(t^2)\right) u' = 0</mrow>
<mrow> \implies \amp \dfrac{du'}{u'} = \left(-4t \dfrac{\cos(t^2)}{\sin(t^2)} + \dfrac{1}{t}\right) dt \implies \ln|u'| = -2 \ln|\sin(t^2)| + \ln t.</mrow>
<mrow> \implies \amp u' = \dfrac{t}{\sin^2(t^2)} \implies u = -\dfrac{1}{2} \cot(t^2) \implies y_2 = -\dfrac{1}{2} \cos(t^2).</mrow>
</md>
By incorporating the <m>-1/2</m> coefficient into the arbitrary constants, we see that the general solution of the ODE is
<me>y = C_1 \sin(t^2) + C_2 \cos(t^2).</me></li>
</ul>
</example>
</subsection>

</section>