<?xml version="1.0" encoding="UTF-8"?>

<section xml:id="sec-2nd-order-linear-gen-theory" xmlns:xi="http://www.w3.org/2001/XInclude">
  <title>General Theories of Second-order Linear ODEs</title>

  <p>From <xref ref="sec-classification"/>, the standard form of a second-order linear ODE is
  <me>y'' + p(t)y' + q(t)y = g(t).</me>
  If <m>g(t) = 0</m>, then the ODE
  <me>y'' + p(t)y' + q(t)y = 0</me>
  is said to be <term>homogeneous</term>. Otherwise, we say the ODE is <term>nonhomogeneous</term>.</p>
  <p>Unlike the first-order ODE where a formula gives the general solution (see <xref ref="sec-1st-order-linear"/>), for second- and higher-order linear ODEs, we do not know how to solve them in general. In this course we will only focus on some <alert>special types</alert> of second-order linear ODEs that appear frequently in science and engineering courses. </p>
  
  <p>We start with some general theories.</p>
  <subsection>
    <title>Existence and Uniqueness Theorem</title>
    <theorem xml:id="th-existence-and-uniqueness-theorem-2nd-order">
      <title>Existence and Uniqueness Theorem</title>
      <statement>
        <p>For the IVP</p>
        <me>y'' + p(t)y' + q(t)y = g(t), \, y(t_0) = y_0, \, y'(t_0) = y_1</me>
        <p>If <m>p(t), q(t), g(t)</m> are continuous in an interval <m>(a, b)</m> that contains <m>t_0</m>, then the IVP has a unique solution on <m>(a, b)</m>.</p>
      </statement>
    </theorem>
    <p>The proof of this theorem is beyond the level of this course. We shall focus on using it. Just like in <xref ref="subsec-existence-uniqueness-2"/>, we may use the theorem to find the interval of existence.</p>
    <example>
      <title>Find the interval of existence of the IVP <m>t^2y'' - 4ty' + 4y = 0, \, y(1) = 1, \, y'(1) = 4</m></title>
      <ul>
        <li>Standard form: <m>y'' - \frac{4}{t}y' + \frac{4}{t^2}y = 0</m></li>
        <li>Singularity: <m>t = 0.</m></li>
      </ul>
      <p>Interval of existence: <m>(0, \infty).</m></p>
    </example>  
    <remark>
      <p>In what follows, all the results are supposed to hold on the interval of existence. </p>
    </remark>
  </subsection>

  <subsection>
    <title>Principle of Superposition</title>
    <theorem xml:id="th-linear-independence-superposition">
      <title>Principle of Superposition</title>
      <statement>
        <ol>
          <li>If <m>y_1, y_2</m> are solutions of a 2<sup>nd</sup>-order linear <em>homogeneous</em> ODE
        <me>y'' + p(t)y' + q(t)y = 0</me>
        then for every real number <m>c_1, c_2</m>, the function
        <me>c_1y_1 + c_2y_2</me>
        is also a solution.</li>
          <li>In addition, if <m>y_1, y_2</m> are linearly independent, i.e., if <m>y_1</m> and <m>y_2</m> are not proportional to each other, then the general solution of the ODE is
        <me>y = c_1y_1 + c_2y_2</me>
      </li>
      </ol>
    </statement>
  </theorem>
<example>
  <title>Check that <m>y_1 = e^{3t}, \, y_2 = e^{-t}</m> are solutions of the ODE <m>y'' - 2y' - 3y = 0.</m> What does the principle of superposition tell us? </title>
  <ol>
  <li><m>y_1 = e^{3t}, \, y_2 = e^{-t}</m> are solutions:
    <me>y_1'' - 2y_1' - 3y_1 = 9e^{3t} - 2 \cdot 3e^{3t} - 3e^{3t} = 0.</me>
    <me>y''_2 - 2y'_2 - 3y_2 = e^{-t} = e^{-t} - 2 \cdot (-e^{-t}) - 3e^{-t} = 0.</me>
  </li>
  <li>
    <m>Y(t) = 20e^{3t} - 99e^{-t} = 20y_1 - 99y_2</m> is also a solution.
    <md>
    <mrow> \amp Y'' - 2Y' - 3Y</mrow>
    <mrow> = \amp (20y_1 - 99y_2)'' - 2(20y_1 - 99y_2)' - 3(20y_1 - 99y_2)</mrow>
    <mrow> = \amp 20y''_1 - 99y''_2 - 2(20y_1' - 99y_2') - 3(20y_1 - 99y_2)</mrow>
    <mrow> = \amp 20y''_1 - 99y''_2 - 2 \cdot 20y_1' + 2 \cdot 99y_2' - 3 \cdot 20y_1 + 3 \cdot 99y_2</mrow>
    <mrow> = \amp 20(y''_1 - 2y'_1 - 3y_1) - 99(y''_2 - 2y_2' - 3y_2)</mrow>
    <mrow> = \amp 20 \cdot 0 - 99 \cdot 0 = 0.</mrow>
    </md>
  </li>
  <li>
    <m>Y(t) = c_1e^{3t} + c_2e^{-t} = c_1y_1 + c_2y_2</m> is also a solution.
    <md>
    <mrow> \amp Y'' - 2Y' - 3Y</mrow>
    <mrow> = \amp (c_1y_1 + c_2y_2)'' - 2(c_1y_1 + c_2y_2)' - 3(c_1y_1 + c_2y_2)</mrow>
    <mrow> = \amp c_1y''_1 + c_2y''_2 - 2 \cdot (c_1y'_1 + c_2y'_2) - 3 \cdot (c_1y_1 + c_2y_2)</mrow>
    <mrow> = \amp c_1y''_1 + c_2y''_2 - 2 \cdot c_1y'_1 - 2 \cdot c_2y'_2 - 3 \cdot c_1y_1 - 3 \cdot c_2y_2</mrow>
    <mrow> = \amp c_1(y''_1 - 2y'_1 - 3y_1) + c_2(y''_2 - 2y'_2 - 3y_2)</mrow>
    <mrow> = \amp c_1 \cdot 0 + c_2 \cdot 0 = 0.</mrow>
    </md>
  </li>
  <li>
    We check that 
    <me>\dfrac{y_1}{y_2} = \dfrac{e^{3t}}{e^{-t}} = e^{4t}</me>
    that is not a constant. So <m>y_1 = e^{3t}</m> and <m>y_2 = e^{-t}</m> are linearly independent, the theorem implies
    <m>y(t) = c_1e^{3t} + c_2e^{-t}</m> is the general solution.
  </li>
</ol>
</example>
<remark>
  <p> The proof of the first part of the superposition principle is not much more difficult than what we did in the example above. I'll leave it as an exercise. The second part, however, is a consequence of <xref ref="th-existence-and-uniqueness-theorem-2nd-order"/>. The proof is not difficult, but for the sake of brevity, we shall not prove it here.</p>
</remark>

</subsection>
<subsection>
  <title>Wronskian for linear independence</title>
  <theorem xml:id="th-wronskian-for-linear-independence">
  <title>Wronskian for linear independence</title>
  <statement>
  <p>If <m>y_1, y_2</m> are solutions of the 2<sup>nd</sup>-order linear homogeneous ODE
  <me>y'' + p(t)y' + q(t)y = 0,</me>
  on an interval where the existence and uniqueness theorem holds, then <m>y_1, y_2</m> are linearly independent if and only if the Wronskian
  <me>(W(y_1, y_2))(t) = \begin{vmatrix} y_1(t) \amp y_2(t) \\ y'_1(t) \amp y'_2(t) \end{vmatrix}</me>
  is nonzero on the interval.</p>
</statement>
</theorem>
<fact>
  <p>It suffices that <m>(W(y_1, y_2))(t) \neq 0</m> on one point of the interval. The proof is not difficult. But for the sake of brevity, we shall not prove it here.</p>
</fact>
<example>
  <title><m>t^2y'' - 4ty' + 6y = 0, \, y_1 = t^2, \, y_2 = t^3.</m></title>
  <p>
  <m>W(y_1, y_2) = \begin{vmatrix} t^2 \amp t^3 \\ 2t \amp 3t^2 \end{vmatrix} = t^4 \neq 0 \text{ as long as } t \neq 0.</m>
</p>
<p>So <m>y_1 = t^2, \, y_2 = t^3</m> are linearly independent.</p>
</example>

<example>
  <title><m>y'' - 9y = 0, \, y_1 = e^{3t}, \, y_2 = 5e^{3t}.</m></title>
  <p>
  <m>W(y_1, y_2) = \begin{vmatrix} e^{3t} \amp 5e^{3t} \\ 3e^{3t} \amp 15e^{3t} \end{vmatrix} = 15e^{6t} - 15e^{6t} = 0.</m>
</p>
<p>So <m>y_1 = e^{3t}, \, y_2 = 5e^{3t}</m> are linearly dependent.</p>
</example>

<example xml:id="ex-wronskian-real-distinct-roots">
  <title><m>ay'' + by' + cy = 0, \, y_1 = e^{r_1 t}, \, y_2 = e^{r_2 t}, \, r_1 \neq r_2.</m></title>
  <p>
  <m>W(y_1, y_2) = \begin{vmatrix} e^{r_1 t} \amp e^{r_2 t} \\ r_1 e^{r_1 t} \amp r_2 e^{r_2 t} \end{vmatrix} = (r_2 - r_1)e^{(r_1 + r_2)t}.</m>
</p>
<p>
  <m>r_1 \neq r_2 \Rightarrow W(y_1, y_2) \neq 0 \Rightarrow \text{Linear independence.}</m>
</p>
</example>
<example>
  <title><m>y'' - \cot(2t)y' = 0, \, y_1 = \sin^2 t, \, y_2 = \cos(2t) - 1.</m></title>
  <p>
  <md>
  <mrow> W(y_1, y_2) = \amp \begin{vmatrix} \sin^2 t \amp \cos(2t) - 1 \\ 2 \sin t \cos t \amp -2 \sin(2t) \end{vmatrix}</mrow>
  <mrow> = \amp -2 \sin^2 t \sin(2t) - (\cos(2t) - 1)2 \sin t \cos t.</mrow>
  </md>
  Set <m>t = \frac{\pi}{4}</m>. Then
  <me> W(y_1, y_2) = -2 \cdot \frac{1}{2} \cdot 1 - (0 - 1) \cdot 2 \cdot \frac{\sqrt{2}}{2} \cdot \frac{\sqrt{2}}{2} = 0.</me>
  So <m>y_1, y_2</m> are <em>linearly dependent.</em></p>
</example>

</subsection>
</section>