<?xml version="1.0" encoding="UTF-8"?>

<section xml:id="sec-2nd-order-linear-const-coeff-real" xmlns:xi="http://www.w3.org/2001/XInclude">
  <title>Second-order Linear ODEs with Constant Coefficients - Real Roots</title>
  <subsection>
    <title>Auxiliary Equation</title>
    <p>Consider the ODE
      <me>ay'' + by' + cy = 0</me>
      where <m>a, b, c</m> are constant numbers. This particular type of ODE can be solved, and are widely used in science and engineering. </p>
    <p>To solve this ODE, we try the function <m>y = e^{rt}.</m> Then
    <me>a(e^{rt})'' + b(e^{rt})' + ce^{rt} = (ar^2 + br + c)e^{rt} = 0.</me>
    This means that if <m>y = e^{rt}</m> is a solution, then necessarily, <m>r</m> is a root of the quadratic equation
    <me>ar^2 + br + c = 0.</me>
    We call it the <term>auxiliary equation</term>.</p>
</subsection>

<subsection>
  <title>The case of two distinct real roots</title>
  <p>If the auxiliary equation has two distinct real roots <m>r_1, r_2</m>, then
    <me>y_1 = e^{r_1 t}, \, y_2 = e^{r_2 t}</me> are solutions, with <m>W(y_1, y_2) \neq 0</m> (see <xref ref="ex-wronskian-real-distinct-roots" />). 
    Then by the <xref ref="th-linear-independence-superposition">principle of superposition</xref>, 
    <me>y = C_1 e^{r_1 t} + C_2 e^{r_2 t}</me> is the general solution.
  </p>


<example>
<title><m>y'' - 2y' - 3y = 0.</m></title>
<p>Auxiliary equation: <m>r^2 - 2r - 3 = 0 \implies r_1 = 3, \, r_2 = -1.</m></p>
<p>General solution: <m>y = C_1 e^{3t} + C_2 e^{-t}.</m></p>
</example>

<example>
<title><m>y'' - 5y' + 6y = 0.</m></title>
<p>Auxiliary equation: <m>r^2 - 5r + 6 = 0 \implies r_1 = 2, \, r_2 = 3.</m></p>
<p>General solution: <m>y = C_1 e^{2t} + C_2 e^{3t}.</m></p>
</example>

<example>
<title><m>y'' - 5y' - 6y = 0.</m></title>
<p>Auxiliary equation: <m>r^2 - 5r - 6 = 0 \implies r_1 = 6, \, r_2 = -1.</m></p>
<p>General solution: <m>y = C_1 e^{6t} + C_2 e^{-t}.</m></p>
</example>

<example>
<title><m>2y'' - 7y' + 3y = 0.</m></title>
<p>Auxiliary equation: <m>2r^2 - 7r + 3 = 0 \implies r_1 = \frac{1}{2}, \, r_2 = 3.</m></p>
<p>General solution: <m>y = C_1 e^{t/2} + C_2 e^{3t}.</m></p>
</example>

</subsection>
<subsection> 
  <title>Initial Value Problems and Long-term behaviors</title>
  <p>Knowing the general solution, we can solve initial value problems and analyze the long-term behavior of the solution. </p>
  <example>
    <title><m>y'' - 4y' - 6y = 0, \, y(0) = 1, \, y'(0) = 0.</m> Find the solution and determine the long-term behavior.</title>
    <ul>
    <li>Auxiliary equation: <m>r^2 - 4r - 6 = 0 \implies r = 2 \pm \sqrt{10}.</m></li> 
    <li>General solution: <m>y = C_1 e^{(2+\sqrt{10})t} + C_2 e^{(2-\sqrt{10})t}.</m></li>
    <li>From the initial values:
    <me>y(0) = 1 \implies C_1 + C_2 = 1</me>
    <me>y'(0) = 1 \implies (2 + \sqrt{10})C_1 + (2 - \sqrt{10})C_2 = 0.</me>
    Solving the system, we obtain
    <me>C_1 = \frac{-5 - \sqrt{10}}{10}, \, C_2 = \frac{5 + \sqrt{10}}{10}.</me>
    </li>
    </ul>
    <p>So the solution is 
    <me>y = \frac{-5 - \sqrt{10}}{10} e^{(2+\sqrt{10})t} + \frac{5 + \sqrt{10}}{10} e^{(2-\sqrt{10})t}.</me>
    As <m>t \to \infty</m>, the second term approaches zero. The solution is dominated by the first term, which approaches <m>- \infty.</m></p>
  </example>

<example>
<title><m>y'' - 5y' + 6y = 0, \, y(0) = \alpha, \, y'(0) = 1.</m> Determine the critical value of <m>\alpha</m> where the long-term behavior changes.</title>
<ul>
<li>Auxiliary equation: <m>r^2 - 5r + 6 = 0 \implies r_1 = 2, \, r_2 = 3.</m></li>
<li>General solution: <m>y = C_1 e^{2t} + C_2 e^{3t}.</m></li>
<li>From the initial values:
<me>y(0) = \alpha \implies C_1 + C_2 = \alpha</me>
<me>y'(0) = 1 \implies 2C_1 + 3C_2 = 1.</me>
Solving the system, we obtain
<me>C_1 = 3\alpha - 1, \, C_2 = 1 - 2\alpha.</me>
</li>
</ul>
<p>So the solution is 
<me>y = (3\alpha - 1)e^{2t} + (1 - 2\alpha)e^{3t}.</me>
As <m>t \to \infty</m>, the solution is dominated by the second term. Note that 
<md>
<mrow>1 - 2\alpha \gt 0 \implies \lim_{t \to \infty} y(t) = +\infty,</mrow>
<mrow>1 - 2\alpha \lt 0 \implies \lim_{t \to \infty} y(t) = -\infty.</mrow>
</md>
Thus, the long-term behavior changes when <m>1 - 2\alpha = 0 \implies \alpha = \frac{1}{2}.</m>
</p>
</example>
</subsection>

</section>