<section xml:id="sec-basic-concepts">
  <title>Basic Concepts</title>

  <definition xml:id="def-diffeq">
    <statement>
      <p>
        A <term>differential equation</term> is an equation concerning derivatives. An <term>ordinary differential equation</term> (abbrev. <term>ODE</term>) is an equation involving only ordinary derivatives of a single-variable function. 
      </p>
    </statement>
  </definition>
  <p>
    Here is the <term>typical form</term> of a first-order ODE: 
  <me>y'(t) = f(t,y(t)).</me>
  or, with the abbreviation of <m>y(t)</m> and <m>y'(t)</m> by <m>y</m> and <m>y'</m>, respectively, 
  <me>y' = f(t,y)</me>
  where</p>
  <ul>
    <li>
      <p><m>t</m> is the independent variable.</p>
    </li>
    <li>
      <p><m>y = y(t)</m> is a one-variable function depending on <m>t</m>.</p>
    </li>
    <li>
      <p><m>y' = \frac{dy}{dt}</m> is the derivative of <m>y</m>.</p>
    </li>
    <li>
      <p><m>f(t,y)</m> is a known function of two variables.</p>
    </li>
  </ul>

  <p>
    This ODE expresses the derivative <m>y'(t)</m> in terms of <m>t</m> and <m>y(t)</m>.
  </p>

  <definition xml:id="def-solution">
    <statement>
      <p>A function <m>y(t)</m> defined on an <alert>open</alert> interval <m>I</m> is called a <term>solution</term> of the ODE <m>y' = f(t,y)</m> on <m>I</m> if</p>
      <ul>
        <li>
          <p><m>y(t)</m> is differentiable on <m>I</m>.</p>
        </li>
        <li>
          <p>For all <m>t</m> in <m>I</m>, the equation <m>y' = f(t,y)</m> holds.</p>
        </li>
      </ul>
    </statement>
  </definition>
  <p>
    While we haven't learned how to solve an ODE, it is easy to check if a function is a solution of an ODE. Simply compute its derivatives, then plug in the ODE, and see if equality holds.
  </p>

  <example xml:id="ex-solution">
    <title>A solution of an ODE</title>
    <p>
      <m>y(t) = e^t</m> is a solution of the ODE <m>y' - y = 0</m>, because <m>y'(t) = e^t</m>, 
    </p>
    <p>
      <m>\implies LHS = y' - y = e^t - e^t = 0 = RHS</m>.
    </p>
    <p>The solution is defined on everywhere on <m>(-\infty, \infty)</m>.</p>
  </example>

  <example xml:id="ex-non-solution">
    <title>A non-solution of an ODE</title>
      <p>
        <m>y(t) = \cos 2t</m> is not a solution of the ODE <m>y' - y = 0</m>, because <m>y'(t) = -2\sin 2t</m>,
      </p>
      <p>
        <m>\implies LHS = y' - y = -2\sin 2t - \cos 2t \neq 0 = RHS</m>.
      </p>
      <p>The solution is defined on everywhere on <m>(-\infty, \infty)</m>.</p>
  </example>

  <remark>
    <p>We shall apply the method of checking solutions extensively in this course, especially in the study of higher-order linear ODEs.</p>
  </remark>
  <definition xml:id="def-general-form">
    <statement>
      <p>
        Most generally, a first-order ODE is of the form
        <me>F(t,y,y') = 0.</me>
        i.e., a relation among the variable <m>t, y,</m> and <m>y'</m>. We call this the <term>general form</term> of a first-order ODE.
      </p>
      <p>The <term>order</term> of a differential equation is the order of the highest derivative appearing in the equation. Similarly, the <term>general form</term> of an <m>n</m>-th order ODE is
      <me>F(t,y,y',...,y^{(n)}) = 0</me>
      i.e., a relation among the variable <m>t, y</m> and the <m>n</m> derivatives <m>y', y'', \cdots, y^{(n)}</m> of <m>y</m>.
  </p>
    </statement>
  </definition>

  
<example>
    <title>Examples of ODEs in typical and general forms</title>
    <statement>
        <p>
            <ul>
                <li><m>y' = t^2 + y</m> (First-order ODE in its typical form).</li>
                <li><m>(y')^2 + \sin y = y + t^2</m> (First-order ODE). </li>
                <li><m>y''' + 3y'' + 3y' + y = e^{2t}</m> (Third-order ODE).</li>
            </ul>
        </p>
    </statement>
</example>

<definition xml:id="def-pde">
  <statement>
    <p>
      A <term>partial differential equation</term> (abbrev. <term>PDE</term>) is an equation concerning partial derivatives. 
    </p>
  </statement>
</definition>

<example>
    <title>Example of a PDE</title>
    <statement>
        <p>
            A harmonic function <m>u = u(x,y)</m> in two variables are defined by the PDE 
            <me>\frac{\partial^2 u}{\partial x^2} + \frac{\partial^2 u}{\partial y^2} = 0.</me>
        </p>
    </statement>
</example>

<p>We shall not require PDEs in this course. </p>
</section>