<?xml version="1.0" encoding="UTF-8"?>

<section xml:id="sec-undetermined-coeff-2" xmlns:xi="http://www.w3.org/2001/XInclude">
  <title>Method of Undetermined Coefficients - Final Ansatz</title>

<subsection>
  <title>The case when the first ansatz fails</title>

<example>
<title> <m>y'' - y' - 2y = e^{2t}</m> with the first ansatz</title>
<ul>
<li> Complementary solution: <m>y_c = C_1e^{-t} + C_2e^{2t}.</m></li>
<li> If we try <m>Y = Ae^{2t},</m> then <m>Y' = 2Ae^{2t}, Y'' = 4Ae^{2t}.</m></li>
<li> Plug the derivatives into the LHS:
<me>Y'' - Y' - 2Y = 2Ae^{2t} - 2Ae^{2t} - 2Ae^{2t} = 0.</me> 
There is no way for <m>Y'' - Y' - 2Y = e^{2t}.</m></li>
</ul>
</example>
<p>Why does this happen? Notice that <m>e^{2t}</m> appears as a part of the complementary solution while my ansatz <m>Ae^{2t}</m> is its constant multiple. When this happens, the first try ansatz fails.</p>

<p>To find a particular solution, we multiply our ansatz by <m>t</m> and try again. </p>
<example>
<title> <m>y'' - y' - 2y = e^{2t}</m> with the second try</title>
<ul>
<li> Set <me>Y = Ate^{2t},</me> then 
<me>Y' = Ae^{2t} + 2Ate^{2t}, Y'' = 4Ae^{2t} + 4Ate^{2t}.</me></li>
<li> Plug the derivatives into the LHS:
<md>
<mrow> \amp Y'' - Y' - 2Y </mrow>
<mrow> = \amp 4Ae^{2t} + 4Ate^{2t} - (Ae^{2t} + 2Ate^{2t}) - 2Ate^{2t}</mrow>
<mrow> = \amp 3Ae^{2t} = e^{2t} </mrow>
</md>
Compare both sides, we see that 
<me>3A = 1 \implies A = \dfrac{1}{3} \implies Y = \dfrac{1}{3}te^{2t}.</me></li>
</ul>
</example>

<example> 
<title> <m>y'' - 2y' + y = 2te^t</m> with the second try fails</title>
<ul>
<li> Complementary solution: <m>y_c = C_1e^t + C_2te^t.</m></li>
<li> The first try ansatz is <m>Y = e^t(At + B) = Ate^t + Be^t.</m></li>
<li> This ansatz clearly fails, as <m>Y</m> has the same structure as the complementary solution. We need to multiply by <m>t.</m></li>
<li> Set <me>Y = te^t(At + B) = (At^2 + Bt)e^t.</me>
Then 
<md> 
<mrow>Y' = \amp (2At + B)e^t + (At^2 + Bt)e^t,</mrow>
<mrow>Y'' = \amp 2Ae^t + 2(2At + B)e^t + (At^2 + Bt)e^t.</mrow>
</md></li>
<li> Plug the derivatives into the LHS:
<md>
<mrow>\amp Y'' - 2Y' + Y</mrow>
<mrow>= \amp 2Ae^t + 2(2At + B)e^t + (At^2 + Bt)e^t</mrow>
<mrow>= \amp - 2((2At + B)e^t + (At^2 + Bt)e^t) + (At^2 + Bt)e^t</mrow>
<mrow>= \amp 2Ae^t.</mrow>
</md>
We do not have <m>te^t</m> terms on the left-hand-side. The equality cannot hold, no matter how <m>A, B</m> are chosen. The second try fails.</li>
</ul>
</example>

<p>To obtain a particular solution, we will have to multiply by another <m>t</m> and try again.</p>

<example> 
<title> <m>y'' - 2y' + y = 2te^t</m> with the third try</title>
<ul>
<li> Now we try:
<me>Y = t^2 e^t(At + B) = (At^3 + Bt^2)e^t.</me>
Then <md>
<mrow>Y' = \amp (3At^2 + 2Bt)e^t + (At^3 + Bt^2)e^t, </mrow>
<mrow>Y'' = \amp (6At + 2B)e^t + 2(3At^2 + 2Bt)e^t + (At^3 + Bt^2)e^t.</mrow>
</md></li>
<li> Plug the derivatives into the LHS:
<md>
<mrow>\amp Y'' - 2Y' + Y</mrow>
<mrow>= \amp (6At + 2B)e^t + 2(3At^2 + 2Bt)e^t + (At^3 + Bt^2)e^t</mrow>
<mrow> \amp - 2((3At^2 + 2Bt)e^t + (At^3 + Bt^2)e^t) + (At^3 + Bt^2)e^t</mrow>
<mrow>= \amp (6At + 2B)e^t = te^t.</mrow>
</md>
Compare both sides, we see that 
<me>6A = 1, 2B = 0 \implies A = \dfrac{1}{6}, B = 0 \implies Y = \dfrac{1}{6}t^3 e^t.</me></li>
</ul>
<p>The general solution:
<me>y = C_1 e^t + C_2 te^t + \dfrac{1}{6}t^3 e^t.</me></p>
</example> 
</subsection>

<subsection>
<title>How to find the final ansatz without trying</title>

<p>Recall: In <m>y'' - y' - 2y = e^{2t}</m> of Example 1:</p>
<ol>
  <li>The aux. eqn. is <m>r^2 - r - 2 = 0 \implies r_1 = 2, r_2 = -1.</m></li>
  <li><m>g(t) = e^{2t}</m> whose exponential coefficient is <m>2,</m> which is a root that appears <alert>once.</alert></li>
  <li>We have seen that the first ansatz failed, the second succeeded.</li>
</ol>

<p>Recall: In <m>y'' - 2y' + y = te^t</m> of Example 2:</p>
<ol>
  <li>The aux. eqn. is <m>r^2 - 2r + 1 = 0 \implies r_1 = r_2 = 1.</m></li>
  <li><m>g(t) = e^t</m> whose exponential coefficient is <m>1,</m> which is a root that appears <alert>twice.</alert></li>
  <li>We have seen that the first and second ansatz failed, the third ansatz succeeded.</li>
</ol>

<p>Generally, for the ODE <m>ay'' + by' + cy = g(t),</m> where</p>
<p><m>g(t) = e^{at} \cos \beta t \cdot (\text{polynomial}) + e^{at} \sin \beta t \cdot (\text{polynomial}),</m></p>
<p>if the complex number <m>\alpha + i\beta</m> appears as a root of the auxiliary equation for <m>m</m> times, then the first <m>m</m> ansatz fail. We should modify the first ansatz by <m>t^m.</m></p>

<remark>
<ol><li>For convenience, we will call the complex number <m>\alpha + i\beta</m> the <term>exponential coefficient</term> of <m>g(t).</m></li> 
<li>The exponential coefficient is a nonstandard terminology. In higher level mathematics, <m>\alpha + i\beta</m> is indeed an eigenvalue with respect to the differential operator. Its associated eigenfunction is <m>e^{(\alpha + i\beta)t}</m> with real part <m>e^{at} \cos \beta t</m> and imaginary part <m>e^{at} \sin \beta t.</m> But it's wrong to call these trigs eigenfunctions.</li>
<li>Since the ODE is <alert>second-order</alert>, there are at most two roots for the auxiliary equation, <alert>the ansatz at most fails twice.</alert></li>
</ol>
</remark>

<example>
<title> <m>y'' + 4y = t \sin 2t.</m></title>
<ul>
<li>Aux. Eqn: <m>r^2 + 4 = 0 \implies r^2 = -4 \implies r = \pm 2i.</m></li>
<li>Complementary solution: <m>y_c = C_1 \cos 2t + C_2 \sin 2t.</m></li>
<li>The first ansatz: <me>Y = (At + B) \cos 2t + (Ct + D) \sin 2t.</me>
Exponential coefficient <m> = 0 + 2i = 2i</m>, a single root. First try fails. The final ansatz should be
<md>
<mrow>Y = \amp t((At + B) \cos 2t + (Ct + D) \sin 2t)</mrow>
<mrow>= \amp (At^2 + Bt) \cos 2t + (Ct^2 + Dt) \sin 2t.</mrow>
</md>
</li>
<li>We use product rule to compute the first derivative:
<md>
<mrow>Y' = \amp (2At + B) \cos 2t - 2(At^2 + Bt) \sin 2t </mrow>
<mrow>\amp + (2Ct + D) \sin 2t + 2(Ct^2 + D) \cos 2t.</mrow>
</md>
To compute <m>Y'',</m> we may use the binomial theorem 
<me>(fg)'' = f''g + 2f'g' + fg''.</me>
Then
<md>
<mrow>Y'' = \amp 2A \cos 2t + 2(2At + B) \cdot (-2 \sin 2t) + (At^2 + Bt) \cdot (-4 \cos 2t) </mrow>
<mrow> \amp + 2C \sin 2t + 2(2Ct + D) \cdot 2 \cos 2t + (Ct^2 + Dt) \cdot (-4 \sin 2t).</mrow>
</md></li>
<li>Plug the derivatives into the LHS:
<md>
<mrow>\amp Y'' + 4Y </mrow>
<mrow> = \amp 2A \cos 2t + 2(2At + B) \cdot (-2 \sin 2t) </mrow>
<mrow> \amp + 2C \sin 2t + 2(2Ct + D) \cdot 2 \cos 2t</mrow>
<mrow> = \amp \cos 2t (8Ct + 2A + 4D) - 2 \sin 2t (-8At - 4B + 2C).</mrow>
<mrow> = \amp \sin 2t.</mrow>
</md>
Comparing the coefficients, we see that
<md>
<mrow>\amp 8C = 0, \quad 2A + 4D = 0, \quad -8A = 1, \quad -4B + 2C = 0</mrow>
<mrow>\implies \amp A = -\dfrac{1}{8}, B = C = 0, D = \dfrac{1}{16}.</mrow>
<mrow>\implies \amp Y = -\dfrac{1}{8}t^2 \cos 2t + \dfrac{1}{16}t \sin 2t.</mrow>
</md></li>
</ul>
<p>The general solution is
<me>y = C_1 \cos 2t + C_2 \sin 2t - \dfrac{1}{8}t^2 \cos 2t + \dfrac{1}{16}t \sin 2t.</me></p>
</example>

<example>
<title> <m>y'' - 2y' + 2y = e^t \cos t.</m></title>
<ul>
<li>Aux. Eqn: <me>r^2 - 2r + 2 = 0 \implies (r - 1)^2 = -1 \implies r = 1 \pm i.</me></li>
<li>Comp. Soln: <me>y_c = C_1 e^t \cos t + C_2 e^t \sin t.</me></li>
<li>First ansatz: <me>Y = Ae^t \cos t + Be^t \sin t.</me>
Exponential coefficient <m>= 1 + i</m> that appear as a single root. First try fails.</li>
<li>Final ansatz: <me>Y = Ate^t \cos t + Bte^t \sin t.</me></li>
<li>To compute the derivatives, we may use the following rules:
<me>(fgh)' = f'g h + f g'h + f g h'.</me>
So
<md>
<mrow>Y' = \amp A(e^t \cos t + te^t \cos t - te^t \sin t) </mrow>
<mrow> \amp + B(e^t \sin t + te^t \sin t + te^t \cos t)</mrow>
<mrow>= \amp ((A + B)t + A)e^t \cos t + ((B - A)t + B)e^t \sin t.</mrow>
<mrow>Y'' = \amp (A + B)e^t \cos t + ((A + B)t + A)e^t \cos t</mrow>
<mrow>\amp + ((A + B)t + A)e^t \cdot (-\sin t) + (B - A)e^t \sin t.</mrow>
<mrow>\amp + ((B - A)t + B)e^t \cos t.</mrow>
<mrow>= \amp ((A + B) + (A + B)t + A + (B - A)t + B)e^t \cos t</mrow>
<mrow> \amp + ((-(A + B)t - A + B - A)t + B)e^t \sin t</mrow>
<mrow>= \amp (2Bt + 2A + 2B)e^t \cos t + (-2At - 2A + 2B)e^t \sin t.</mrow>
</md>
</li>
<li>Plug the derivatives into the LHS:
<md>
<mrow>\amp Y'' - 2Y' + 2Y</mrow>
<mrow>= \amp (2Bt + 2A + 2B - 2((A + B)t + A) + 2At)e^t \cos t</mrow>
<mrow> \amp + (-2At - 2A + 2B - 2((B - A)t + B) + 2Bt)e^t \sin t</mrow>
<mrow>= \amp 2Be^t \cos t - 2Ae^t \sin t = e^t \cos t.</mrow>
</md>
Comparing the coefficients, we see that
<me>2B = 1, -2A = 0 \implies A = 0, B = \dfrac{1}{2} \implies Y = \dfrac{1}{2}te^t \sin t.</me>
</li>
</ul>
<p>The general solution is
<me>y = C_1 e^t \cos t + C_2 e^t \sin t + \dfrac{1}{2} te^t \sin t.</me></p>
</example>

<remark>
<p> There does exist faster ways to compute everything by hand. In the MIT Lecture 13 and 14, there exists a simpler way of computing <m>Y'' - 2Y' + 2Y</m>, using the exponential shift lemma of differential operators and complex functions. We shall not require that in our course. </p>
</remark>
</subsection>

<subsection>
<title>Sums of functions with different exponential coefficients.</title>

<p>We have seen how to solve <m>ay'' + by' + cy = g(t)</m> when
<me>g(t) = e^{\alpha t} \cos \beta t \cdot (\text{polynomial}) + e^{\alpha t} \sin \beta t \cdot (\text{polynomial}).</me>
We use the exponential coefficient <m>\alpha + i\beta</m> to determine the final ansatz. </p>

<p>What shall we do if <m>g(t)</m> is a sum of such functions but with different <m>\alpha</m>'s and <m>\beta</m>'s? For example,
<me>g(t) = t^3 + e^t + \sin 2t + 2 \cos 2t.</me>
To handle such <m>g(t),</m> we need the following <alert>principle of superposition</alert>.</p>

<theorem>
<title>Principle of superposition: nonhomogeneous ODEs</title>
<statement>
<p>Let <m>Y_1</m> be a particular solution of
<me>y'' + p(t)y' + q(t)y = g_1(t),</me>
and <m>Y_2</m> be a particular solution of
<me>y'' + p(t)y' + q(t)y = g_2(t).</me>
Then <m>Y_1 + Y_2</m> is a particular solution of
<me>y'' + p(t)y' + q(t)y = g_1(t) + g_2(t).</me></p>
</statement>
</theorem>

<proof>
<p>The assumption implies that
<me>Y_1'' + p(t)Y_1' + q(t)Y_1 = g_1(t),</me>
<me>Y_2'' + p(t)Y_2' + q(t)Y_2 = g_2(t).</me>
Adding them up, by linearity of differential operators, we have
<me>(Y_1 + Y_2)'' + p(t)(Y_1 + Y_2)' + q(t)(Y_1 + Y_2) = g_1(t) + g_2(t).</me>
Thus <m>Y_1 + Y_2</m> satisfies the ODE
<me>y'' + p(t)y' + q(t)y = g_1(t) + g_2(t).</me></p>
</proof>

<p>From the principle of superposition, we know that to handle such <m>g(t):</m></p>
<ol>
  <li>Break <m>g(t) = g_1(t) + \cdots + g_m(t),</m> according to the exponential coefficients.</li>
  <li>Find <m>Y_1, \ldots, Y_m</m> individually for <m>g_1, \ldots, g_m,</m> i.e., for <m>i = 1, \ldots, m,</m> find a particular <m>Y_i</m> for <m>ay'' + by' + cy = g_i(t).</m></li>
  <li>Then <m>Y = Y_1 + \cdots + Y_m</m> is a particular solution.</li>
</ol>

<example>
<title> <m>y'' + y = t + t \sin t + 2 \cos t.</m></title>
<ul>
<li>Aux. Eqn: <m>r^2 + 1 = 0 \implies r = \pm i.</m></li>
<li>Comp. Soln: <m>y_c = C_1 \cos t + C_2 \sin t.</m></li>
<li>Now we regard <m>g(t) = g_1(t) + g_2(t),</m> where
<md>
<mrow>g_1(t) = \amp t,</mrow>
<mrow>g_2(t) = \amp t \sin t + 2 \cos t.</mrow>
</md>
(Note: Terms with the same exponential coefficient should be collected together to avoid unnecessary repetitions.)</li>
<li>First we deal with <m>g_1(t) = t.</m> The first ansatz is <me>Y_1 = At + B.</me> The exponential coefficient is <m>0</m> that is not a root. First ansatz succeeds.</li>
<li> We calculate the derivatives and plug them into the LHS
<md>
<mrow>\amp Y_1' = A, \quad Y_1'' = 0 \implies Y_1'' + Y_1 = At + B = g_1(t) = t</mrow>
<mrow>\implies \amp A = 1, B = 0 \implies Y_1 = t.</mrow>
</md>
</li>
<li> For <m>g_2(t)</m>, the first ansatz is <me>Y_2 = (Ct + D) \cos t + (Et + F) \sin t.</me>
The exponential coefficient is <m>i</m> that appears as a single root. First try fails. The final ansatz is
<me>Y_2 = (Ct^2 + Dt) \cos t + (Et^2 + Ft) \sin t.</me></li>
<li>We compute the derivatives and find that
<md>
<mrow> \amp Y_2'' + Y_2 </mrow>
<mrow> = \amp (-4Ct + 2E - 2D) \sin t + (4Et + 2F + 2C) \cos t.</mrow>
<mrow> = \amp t \sin t + 2 \cos t.</mrow>
</md>
Compare the coefficients, we see that
<md>
<mrow> \amp -4C = 1, \quad 2E - 2D = 0, \quad 4E = 0, \quad 2F + 2C = 2.</mrow>
<mrow> \amp \implies C = -\dfrac{1}{4}, \quad D = E = 0, \quad F = \dfrac{5}{4}.</mrow>
<mrow> \amp \implies Y_2 = -\dfrac{1}{4}t^2 \cos t + \dfrac{5}{4}t \sin t.</mrow>
</md>
</li>
<li>From the principle of superposition,
<me>Y = Y_1 + Y_2 = t - \dfrac{1}{4}t^2 \cos t + \dfrac{5}{4}t \sin t</me>
is a particular solution of the ODE. </li>
</ul>
<p> The general solution is then
<me>y = C_1 \cos t + C_2 \sin t + t - \dfrac{1}{4}t^2 \cos t + \dfrac{5}{4}t \sin t.</me></p> 
</example>

<remark>
<p> A computer can easily handle the derivatives. But to make sure the computer is doing the right thing, it is important for us human to know the correct ansatz at the very least. We will not be able to figure out a mistake made by a computer if we do not know what we are expecting and cannot perform the simplest calculation. This is the main emphasis of this section. </p>
</remark>

</subsection>
</section>