<?xml version="1.0" encoding="UTF-8"?>

<section xml:id="sec-2nd-order-linear-non-homogeneous" xmlns:xi="http://www.w3.org/2001/XInclude">
  <title>Second-order Linear Non-Homogeneous ODEs</title>

<subsection>
<title>Principle of Superposition and the Structure of the General Solution</title>
<p>The general solution of a nonhomogeneous linear ODE</p>
<me>y'' + p(t)y' + q(t)y = g(t)</me>
<p>is closely related to the solution of the homogeneous ODE</p>
<me>y'' + p(t)y' + q(t)y = 0.</me>

<theorem xml:id="thm-superposition-nonhomogeneous">
<title>Principle of Superposition</title>
<statement>
<p>Let <m>Y_1, Y_2</m> be two solutions of <me>y'' + p(t)y' + q(t)y = g(t).</me> Then <m>Y_1 - Y_2</m> is a solution of <me>y'' + p(t)y' + q(t)y = 0.</me></p>
</statement>
</theorem>

<proof>
<p>The assumption states that
<me>Y_1'' + p(t)Y_1' + q(t)Y_1 = g(t),</me>
and 
<me>Y_2'' + p(t)Y_2' + q(t)Y_2 = g(t).</me>
Subtract these two equations, by linearity of derivatives, we get
<me>(Y_1 - Y_2)'' + p(t)(Y_1 - Y_2)' + q(t)(Y_1 - Y_2) = 0.</me>
Thus <m>Y_1 - Y_2</m> is a solution of the <m>y'' + p(t)y' + q(t)y = 0.</m></p>
</proof>

<theorem>
<title>Structure of the general solution</title>
<statement>
<p>The general solution of <m>y'' + p(t)y' + q(t)y = g(t)</m> is of the form
<me>y = y_c + Y = C_1y_1 + C_2y_2 + Y</me>
where</p> 
<ul>
<li><m>y_c = C_1y_1 + C_2y_2</m> is the general solution of the homogeneous ODE
<me>y'' + p(t)y' + q(t)y = 0.</me></li>
<li><m>Y</m> is a particular solution of ODE <me>y'' + p(t)y' + q(t)y = g(t).</me></li>
</ul>
</statement>
</theorem>

<proof> 
<p>We first check that <m>y = y_c + Y</m> is a solution:
<md>
<mrow>LHS \amp= (y_c + Y)'' + p(t)(y_c + Y)' + q(t)(y_c + Y)</mrow>
<mrow>\amp= y_c'' + p(t)y_c' + q(t)y_c + Y'' + p(t)Y' + q(t)Y</mrow>
<mrow>\amp= 0 + g(t) = RHS.</mrow>
</md></p>
<p>It remains to check that <alert>any solution is of this form.</alert> Let <m>y</m> be any solution of the nonhomogeneous ODE. Then from the <xref ref="thm-superposition-nonhomogeneous"/>, <m>y - Y</m> is a solution of the homogeneous ODE. Thus
<me>y - Y = C_1y_1 + C_2y_2</me>
for some numbers <m>C_1, C_2.</m> In other words, <me>y = C_1y_1 + C_2y_2 + Y.</me></p>
</proof>

<definition>
<p><m>y_c = C_1y_1 + C_2y_2</m> is called the <term>complementary solution</term> <m>Y</m> is called a <term>particular solution</term>.</p>
</definition>

<p>Solving a nonhomogeneous ODE reduces to two parts: Solve the homogeneous ODE to find the complementary solution, then find a particular solution.</p>
</subsection>

<subsection>
<title>Linear ODE with constant coefficients</title>

<p>For a second order linear nonhomogeneous ODE with constant coefficients
<me>ay'' + by' + cy = g(t),</me>
we learned how to find the complementary solution:</p>
<p>We start by forming the auxiliary equation <m>ar^2 + br + c = 0</m> and solve the quadratic equation. Three cases:</p>
<ul>
  <li>Two distinct real roots <m>r_1 \neq r_2,</m> <m>y_c = C_1e^{r_1t} + C_2e^{r_2t}.</m></li>
  <li>Two distinct complex roots <m>r_1 = \alpha + i\beta, r_2 = \alpha - i\beta,</m> <m>y_c = C_1e^{\alpha t} \cos \beta t + C_2e^{\alpha t} \sin \beta t.</m></li>
  <li>Two repeated real roots <m>r_1 = r_2 = r,</m> <m>y_c = C_1e^{rt} + C_2te^{rt}.</m></li>
</ul>

<p>For a second order linear nonhomogeneous ODE with constant coefficients
<me>ay'' + by' + cy = g(t),</me>
There are two approaches of finding a particular solution.</p>
<ol>
  <li>Method of Undetermined Coefficients. The method is convenient and easy to generalize to higher-order linear ODEs, but only works when all the coefficients are constant and <m>g(t)</m> ranges in special classes of functions. Nevertheless, these special cases are good enough for lots of engineering practices.</li>
  
  <li><p> Variation of Parameter <alert>(not required).</alert> Knowing the complementary solution <m>y_c = C_1y_1 + C_2y_2,</m> we may set <m>Y = u_1y_1 + u_2y_2</m> and solve that
  <me>Y = y_1 \cdot \int \dfrac{-y_2 \cdot g}{W(y_1, y_2)} dt + y_2 \cdot \int \dfrac{y_1 \cdot g}{W(y_1, y_2)} dt</me>
  Therefore, knowing one part of the complementary solution, we may apply the reduction of order in <xref ref="sec-2nd-order-linear-const-coeff-repeated-2"/> to find the full complementary solution, then use this formula to find the particular solution. </p>
  <p>While this integration formula is powerful and can be generalized to higher-order linear ODEs, the formula in higher-order case is much more complicated and not so convenient to use. </p> 
  </li>
</ol>

</subsection>
</section>