<?xml version="1.0" encoding="UTF-8"?>

<section xml:id="sec-higher-order-linear-ODEs" xmlns:xi="http://www.w3.org/2001/XInclude">
  <title>Higher-order Linear ODEs</title>
<p><strong>Higher order linear ODE – General theory</strong></p>

<ol>
  <li>Homogeneous case: For the ODE</li>
  <p><m>y^{(n)} + p_1(t)y^{(n-1)} + \cdots + p_{n-1}(t)y' + p_n(t)y = 0</m></p>
  <ul>
    <li>Fundamental set of solutions: <m>y_1, \ldots, y_n</m> that are
      <ul>
        <li>solutions of the ODE;</li>
        <li>linear independent, i.e., the Wronskian</li>
      </ul>
      <p><m>W(y_1, \ldots, y_n) = \begin{vmatrix}
        y_1 \amp \cdots \amp y_n \\
        \vdots \amp \ddots \amp \vdots \\
        y_1^{(n-1)} \amp \cdots \amp y_n^{(n-1)}
      \end{vmatrix}</m> is nowhere vanishing (won’t require).</p>
    </li>
    
    <li>Principle of superposition: If <m>y_1, \ldots, y_n</m> forms a fundamental set of solutions, then the general solution of the ODE is <m>y = C_1y_1 + \cdots + C_ny_n.</m></li>
  </ul>
</ol>
<p><strong>2. Nonhomogeneous case:</strong> For the ODE</p>
<p><m>y^{(n)} + p_1(t)y^{(n-1)} + \cdots + p_{n-1}(t)y' + p_n(t)y = g(t)</m></p>

<ul>
  <li>Structure of general solution: <m>y = y_c + Y,</m> where
    <ul>
      <li><m>y_c,</m> the <span style="color:magenta;">complementary solution,</span> is the general solution of the homogeneous ODE.</li>
      <li><m>Y,</m> a particular solution, is a solution of the nonhomogeneous ODE.</li>
    </ul>
  </li>

  <li>Principle of superposition:
    <ul>
      <li>If <m>Y_1</m> is a solution of <m>y^{(n)} + \cdots + p_n(t)y = g_1(t),</m></li>
      <li><m>Y_2</m> is a solution of <m>y^{(n)} + \cdots + p_n(t)y = g_2(t),</m></li>
      <li>then <m>Y_1 + Y_2</m> is a solution of <m>y^{(n)} + \cdots + p_n(t)y = g_1(t) + g_2(t).</m></li>
    </ul>
  </li>
</ul>

<p><strong>Higher order linear ODE with Const. Coeff.</strong></p>

<ol>
  <li>Homogeneous case: For the ODE,</li>
  <p><m>a_ny^{(n)} + a_{n-1}y^{(n-1)} + \cdots + a_1y' + a_0y = 0</m></p>
  <p>We try <m>y = e^{rt}</m> and see that</p>
  <p><m>a_n r^n e^{rt} + a_{n-1} r^{n-1} e^{rt} + \cdots + a_1 r e^{rt} + a_0 e^{rt} = 0.</m></p>
  <p>Dividing by <m>e^{rt},</m> we obtain the <span style="color:magenta;">auxiliary equation</span></p>
  <p><m>a_n r^n + a_{n-1} r^{n-1} + \cdots + a_1 r + a_0 = 0.</m></p>
</ol>

<p><strong>Theorem:</strong> Every polynomial with real coefficients can be factored as a product of linear and quadratic polynomials.</p>

<p><strong>Corollary:</strong> If <m>\alpha + i\beta</m> is a root that is repeated <m>m</m> times, then its conjugate <m>\alpha - i\beta</m> is also a root that is repeated <m>m</m> times.</p>
<p>Let <m>r</m> be a solution of the auxiliary equation.</p>

<p><strong>Case 1:</strong> If <m>r</m> is a real <span style="color:red;">single</span> root, then it contributes <span style="color:red;">one</span> function <m>e^{rt}</m> to the fundamental set of solutions.</p>

<p><strong>Case 2:</strong> If <m>r</m> is a real root repeated <m>m</m> times, then it contributes <m>m</m> functions</p>
<p><m>e^{rt}, \, te^{rt}, \ldots, \, t^{m-1}e^{rt},</m></p>
<p>to the fundamental set of solutions.</p>

<p><strong>Case 3:</strong> If <m>r = \alpha + i\beta</m> is a complex single root, then together with its conjugate <m>\bar{r} = \alpha - i\beta,</m> they contribute <span style="color:red;">two</span> functions</p>
<p><m>e^{\alpha t} \cos \beta t, \, e^{\alpha t} \sin \beta t</m> to the fundamental set of solutions.</p>

<p><strong>Case 4:</strong> If <m>r = \alpha + i\beta</m> is a complex root repeated <m>m</m> times, then together with <m>\bar{r} = \alpha - i\beta,</m> they contribute <span style="color:red;">2m</span> functions</p>
<p><m>e^{\alpha t} \cos \beta t, \, e^{\alpha t} \sin \beta t, \, te^{\alpha t} \cos \beta t, \, te^{\alpha t} \sin \beta t, \, \ldots, \, t^{m-1}e^{\alpha t} \cos \beta t, \, t^{m-1}e^{\alpha t} \sin \beta t,</m></p>
<p>to the fundamental set of solutions.</p>

<p><strong>Example 1:</strong> <m>y''' - y' = 0.</m></p>
<p>Auxiliary equation: <m>r^3 - r = 0 \implies r(r^2 - 1) = 0 \implies r(r - 1)(r + 1) = 0 \implies r_1 = -1, r_2 = 0, r_3 = 1.</m></p>
<p>General solution: <m>y = C_1 e^{-t} + C_2 + C_3 e^t.</m></p>

<p><strong>Example 2:</strong> <m>y''' - y'' - y' + y = 0.</m></p>
<p>Auxiliary equation: <m>r^3 - r^2 - r + 1 = 0</m></p>
<p><m>LHS = r^2(r - 1) - (r - 1) = (r - 1)(r^2 - 1) = (r - 1)(r - 1)(r + 1) \implies r_1 = -1, r_2 = r_3 = 1.</m></p>
<p>General solution: <m>y = C_1 e^{-t} + C_2 e^t + C_3 t e^t.</m></p>

<p><strong>Example 3:</strong> <m>y''' - 3y'' + 3y - y = 0.</m></p>
<p>Auxiliary equation: <m>r^3 - 3r^2 + 3r - 1 = 0</m></p>
<p><m>LHS = r^3 - 1 - 3r(r - 1) = (r - 1)(r^2 + r + 1) - 3r(r - 1)</m></p>
<p><m>= (r - 1)(r^2 + r + 1 - 3) = (r - 1)(r^2 - 2r + 1)</m></p>
<p><m>= (r - 1)^3 = 0 \implies r_1 = r_2 = r_3 = 1.</m></p>
<p>General solution: <m>y = C_1 e^t + C_2 te^t + C_3 t^2 e^t.</m></p>

<p><strong>Example 4:</strong> <m>y''' - y = 0.</m></p>
<p>Auxiliary equation: <m>r^3 - 1 = 0 \implies (r - 1)(r^2 + r + 1) = 0</m></p>
<p><m>\implies r_1 = 1, r_2 = -\dfrac{1}{2} + \dfrac{\sqrt{3}}{2} i, r_3 = -\dfrac{1}{2} - \dfrac{\sqrt{3}}{2} i.</m></p>

<p>General solution:</p>
<p><m>y = C_1 e^t + C_2 e^{-\frac{t}{2}} \cos\left(\dfrac{\sqrt{3}}{2} t\right) + C_3 e^{-\frac{t}{2}} \sin\left(\dfrac{\sqrt{3}}{2} t\right).</m></p>

<p><strong>Example 5:</strong> <m>y^{(4)} + 8y'' + 16y = 0.</m></p>
<p>Auxiliary equation: <m>r^4 + 8r^2 + 16 = 0</m></p>
<p><m>\implies (r^2 + 4)^2 = 0 \implies r_1 = r_2 = 2i, r_3 = r_4 = -2i.</m></p>
<p>General solution:</p>
<p><m>y = C_1 \cos 2t + C_2 \sin 2t + C_3 t \cos 2t + C_4 t \sin 2t.</m></p>

<p><strong>Example 6:</strong> <m>y^{(4)} + 4y = 0.</m></p>
<p>Auxiliary equation: <m>r^4 + 4 = 0.</m> So <m>r = 4^{1/4} \sqrt{-1}.</m></p>
<p>Recall that</p>
<p><m>4^{1/4} = (4e^{i(\pi + 2k\pi)})^{1/4} = 2 \cdot 2^{1/4} e^{i(\frac{\pi}{4} + \frac{k\pi}{2})}.</m></p>
<p>Thus <m>r_1 = \sqrt{2} e^{i \frac{\pi}{4}} = \sqrt{2} \left( \cos \frac{\pi}{4} + i \sin \frac{\pi}{4} \right) = 1 + i,</m></p>
<p><m>r_2 = \sqrt{2} e^{i \frac{3\pi}{4}} = \sqrt{2} \left( \cos \frac{3\pi}{4} + i \sin \frac{3\pi}{4} \right) = -1 + i.</m></p>

<p><strong>Example 6:</strong> <m>y^{(4)} + 4y = 0.</m></p>
<p>Auxiliary equation: <m>r^4 + 4 = 0.</m> So <m>r = 4^{1/4} \sqrt{-1}.</m></p>
<p>Recall that</p>
<p><m>4^{1/4} = (4e^{i(\pi + 2k\pi)})^{1/4} = 2 \cdot 2^{1/4} e^{i(\frac{\pi}{4} + \frac{k\pi}{2})}.</m></p>

<p>Thus</p>
<p><m>r_1 = \sqrt{2} e^{i \frac{\pi}{4}} = \sqrt{2} \left( \cos \frac{\pi}{4} + i \sin \frac{\pi}{4} \right) = 1 + i,</m></p>
<p><m>r_2 = \sqrt{2} e^{i \frac{3\pi}{4}} = \sqrt{2} \left( \cos \frac{3\pi}{4} + i \sin \frac{3\pi}{4} \right) = -1 + i,</m></p>
<p><m>r_3 = \sqrt{2} e^{i \frac{5\pi}{4}} = \sqrt{2} \left( \cos \frac{5\pi}{4} + i \sin \frac{5\pi}{4} \right) = -1 - i,</m></p>
<p><m>r_4 = \sqrt{2} e^{i \frac{7\pi}{4}} = \sqrt{2} \left( \cos \frac{7\pi}{4} + i \sin \frac{7\pi}{4} \right) = 1 - i.</m></p>

<p><strong>General solution:</strong></p>
<p><m>y = C_1 e^t \cos t + C_2 e^t \sin t + C_3 e^{-t} \cos t + C_4 e^{-t} \sin t.</m></p>

<p><strong>Higher order linear ODE with Const. Coeff.</strong></p>

<ol>
  <li>Nonhomogeneous case: For the ODE</li>
  <p><m>a_n y^{(n)} + a_{n-1} y^{(n-1)} + \cdots + a_1 y' + a_0 y = g(t)</m></p>
  <p>Variation of parameters would be quite complicated. But the method of coefficients works in the same way.</p>

  <p>Step 1: Separate <m>g(t)</m> according to exponential coefficients, i.e., write <m>g(t) = g_1(t) + g_2(t) + \cdots + g_m(t),</m> where each <m>g_j(t)</m> is of the form:</p>
  <p><m>g_j(t) = e^{\alpha_j t} \cos \beta_j t \, (\text{polynomial}) + e^{\alpha_j t} \sin \beta_j t \, (\text{polynomial}),</m></p>
  <p>For example, if <m>g(t) = te^t + 3 \cos 3t + t^2 + 4t \sin 3t + 2t^2 e^t + 1</m></p>
  <p>we should write <m>g(t) = g_1(t) + g_2(t) + g_3(t),</m> where</p>
  <p><m>g_1(t) = (2t^2 + t)e^t, \, g_2(t) = 3 \cos 3t + 4t \sin 3t, \, g_3(t) = t^2 + 1.</m></p>
</ol>
<p><strong>Step 2:</strong> We find a particular solution <m>Y_j</m> for each</p>
<p><m>g_j(t) = e^{\alpha_j t} \cos \beta_j t \, (\text{polynomial}) + e^{\alpha_j t} \sin \beta_j t \, (\text{polynomial}).</m></p>
<p>The first ansatz should be set as</p>
<p><m>Y_j = e^{\alpha_j t} \cos \beta_j t (A_n t^n + \cdots + A_0) + e^{\alpha_j t} \sin \beta_j t (B_n t^n + \cdots + B_0).</m></p>
<p>where <m>n</m> is the largest degree appearing in the polynomial.</p>
<p>If the exponential coefficient <m>\alpha_j + i\beta_j</m> does not appear as a root of the auxiliary equation, the first ansatz succeeds.</p>
<p>If <m>\alpha + i\beta</m> is a root repeated <m>m</m> times, the final ansatz should be modified by <m>t^m,</m> i.e.,</p>
<p><m>Y = t^m \, (\text{First Ansatz}).</m></p>

<p><strong>Step 3:</strong> Once we find a particular solution for each</p>
<p><m>g_j(t) = e^{\alpha_j t} \cos \beta_j t \, (\text{polynomial}) + e^{\alpha_j t} \sin \beta_j t \, (\text{polynomial}),</m></p>
<p>the principle of superposition implies that</p>
<p><m>Y = Y_1 + Y_2 + \cdots + Y_m</m></p>
<p>is a particular solution of the nonhomogeneous ODE.</p>
<p><m>a_n y^{(n)} + a_{n-1} y^{(n-1)} + \cdots + a_1 y' + a_0 y = g(t)</m></p>
<p>for <m>g(t) = g_1(t) + g_2(t) + \cdots + g_m(t).</m></p>

<p>If you wish to ask the computer to carry out the calculation, make sure you plug in the final ansatz for each <m>Y_j</m> in <m>Y.</m></p>

<p><strong>Example 7:</strong> Determine the final ansatz for the following ODES.</p>

<p>(a) <m>y''' - y'' - y' + y = 2e^{-t}.</m></p>
<p>Aux. eqn: <m>r^3 - r^2 - r + 1 = (r - 1)^2(r + 1) = 0 \implies r = -1, 1, 1.</m></p>
<p>The first ansatz <m>Y = Ae^{-t}.</m> Exp. Coeff. = <m>-1,</m> single root.</p>
<p>The final ansatz <m>Y = Ate^{-t}.</m></p>

<p>(b) <m>y''' - y'' - y' + y = 2e^t.</m></p>
<p>Solutions of the Aux. eqn: <m>r = -1, 1, 1.</m></p>
<p>The first ansatz <m>Y = Ae^t.</m> Exp. Coeff. = <m>1,</m> double root.</p>
<p>The final ansatz <m>Y = At^2 e^t.</m></p>

<p>(c) <m>y^{(4)} - y = \cos t.</m></p>
<p>Aux. eqn: <m>r^4 - 1 = (r - 1)(r + 1)(r^2 + 1) = 0 \implies r = -1, 1, i, -i.</m></p>
<p>First ansatz <m>Y = A \cos t + B \sin t.</m> Exp. Coeff. = <m>i,</m> single root.</p>
<p>Final ansatz <m>Y = At \cos t + Bt \sin t.</m></p>

<p>(d) <m>y^{(4)} + 2y'' + y = t \sin t.</m></p>
<p>Aux. eqn: <m>r^4 + 2r^2 + 1 = (r^2 + 1)^2 = 0 \implies r = i, -i, -i, i.</m></p>
<p>First ansatz <m>Y = \cos t (At + B) + \sin t (Ct + D).</m></p>
<p>Exp. Coeff. = <m>i</m> that is a double root.</p>
<p>Final ansatz <m>Y = \cos t (At^3 + Bt^2) + \sin t (Ct^3 + Dt^2).</m></p>

<p>(e) <m>y^{(4)} + 2y''' + 2y'' = 16.</m></p>
<p>Aux. Eqn. <m>r^4 + 2r^3 + 2r^2 = 0 \implies r^2(r^2 + 2r + 2) = 0</m> 
  <m>\implies r_1 = r_2 = 0, r_3 = -1 + i, r_4 = -1 - i.</m></p>
<p>First ansatz <m>Y = A.</m> Exp. Coeff. = <alert>0</alert>, double root.</p>
<p>Final ansatz <m>Y = At^2.</m></p>

<p>(f) <m>y^{(4)} + 2y''' + 2y'' = e^{-t} \cos t.</m></p>
<p>Aux. eqn. <m>r^4 + 2r^3 + 2r^2 = r^2(r^2 + 2r + 2) = 0</m> 
  <m>\implies r = 0, -1 + i, -1 - i.</m></p>
<p>First ansatz <m>Y = Ae^{-t} \cos t + Be^{-t} \sin t.</m></p>
<p>Exp. Coeff. = <alert>-1 + i</alert> that is a single root.</p>
<p>Final ansatz <m>Y = Ate^{-t} \cos t + Bte^{-t} \sin t.</m></p>

<p>Example 8: Find the general solution of</p>
<p><m>y''' - y'' - y' + y = 8e^t + 4e^{-t} + 25 \cos 2t + t^2.</m></p>

<p>Aux. Eqn. <m>r^3 - r^2 - r + 1 = r^2(r - 1) - (r - 1) = (r - 1)(r^2 - 1) = (r - 1)^2(r + 1) = 0</m> 
  <m>\implies r = -1, 1, 1.</m></p>

<p>Comp. Soln. <m>y_c = C_1 e^{-t} + C_2 e^t + C_3 t e^t.</m></p>
<p>Let <m>Y_1</m> be a solution of <m>y''' - y'' - y' + y = 8e^t.</m></p>
<p>First ansatz <m>Y_1 = Ae^t.</m> Exp. Coeff. = <alert>1</alert> which is a double root.</p>
<p>Final ansatz <m>Y_1 = At^2 e^t.</m> Then <m>Y'_1 = 2Ate^t + At^2 e^t,</m></p>
<p><m>Y''_1 = 2Ae^t + 2Ate^t + 2Ate^t = 2Ae^t + 4Ate^t + At^2 e^t,</m></p>
<p><m>Y'''_1 = 2Ae^t + 4A(e^t + te^t) + 2Ate^t = 6Ae^t + 6Ate^t.</m></p>
<p><m>Y'''_1 - Y''_1 - Y'_1 + Y_1 = 6Ae^t + 6Ate^t + At^2 e^t - (2Ae^t + 4Ate^t + At^2 e^t)</m></p>
<p><m> - (2Ate^t + At^2 e^t) + At^2 e^t = 4Ae^t = 8e^t \implies A = 2.</m></p>
<p>So <m>Y_1 = 2t^2 e^t.</m></p>

<p>Let <m>Y_2</m> be a solution of <m>y''' - y'' - y' + y = 4e^{-t}.</m></p>
<p>First ansatz <m>Y_2 = Be^{-t}.</m> Exp. Coeff. = <alert>-1</alert> which is a single root.</p>
<p>Final ansatz <m>Y_2 = Bte^{-t}.</m> Then <m>Y'_2 = Be^{-t} - Bte^{-t},</m></p>
<p><m>Y''_2 = -Be^{-t} - (Be^{-t} - Bte^{-t}) = -2Be^{-t} + Bte^{-t},</m></p>
<p><m>Y'''_2 = 2Be^{-t} + Be^{-t} - Bte^{-t} = 3Be^{-t} - Bte^{-t}.</m></p>
<p><m>Y'''_2 - Y''_2 - Y'_2 + Y_2 = 3Be^{-t} - (-2Be^{-t} + Bte^{-t}) - (-Be^{-t} - Bte^{-t})</m></p>
<p><m> = - (Be^{-t} - Bte^{-t}) + Bte^{-t} = 4Be^{-t} = 4e^{-t} \implies B = 1.</m></p>
<p>So <m>Y_2 = te^{-t}.</m></p>

<p>Let <m>Y_2</m> be a solution of <m>y''' - y'' - y' + y = 4e^{-t}.</m></p>
<p>First ansatz <m>Y_2 = Be^{-t}.</m> Exp. Coeff. = <alert>-1</alert> which is a single root.</p>
<p>Final ansatz <m>Y_2 = Bte^{-t}.</m> Then <m>Y'_2 = Be^{-t} - Bte^{-t},</m></p>
<p><m>Y''_2 = -Be^{-t} - (Be^{-t} - Bte^{-t}) = -2Be^{-t} + Bte^{-t},</m></p>
<p><m>Y'''_2 = 2Be^{-t} + Be^{-t} - Bte^{-t} = 3Be^{-t} - Bte^{-t}.</m></p>
<p><m>Y'''_2 - Y''_2 - Y'_2 + Y_2 = 3Be^{-t} - (-2Be^{-t} + Bte^{-t}) - (-Be^{-t} - Bte^{-t})</m></p>
<p><m> = - (Be^{-t} - Bte^{-t}) + Bte^{-t} = 4Be^{-t} = 4e^{-t} \implies B = 1.</m></p>
<p>So <m>Y_2 = te^{-t}.</m></p>

<p>Let <m>Y_3</m> be a solution of <m>y''' - y'' - y' + y = 25 \cos 2t.</m></p>
<p>First ansatz <m>Y_3 = C \cos 2t + D \sin 2t.</m></p>
<p>Exp. Coeff. = <alert>2i</alert>, not a root. <m>Y'_3 = -2C \sin 2t + 2D \cos 2t,</m></p>
<p><m>Y''_3 = -4C \cos 2t - 4D \sin 2t,</m> <m>Y'''_3 = 8C \sin 2t - 8D \cos 2t.</m></p>
<p><m>Y'''_3 - Y''_3 - Y'_3 + Y_3 = 8C \sin 2t - 8D \cos 2t - (-4C \cos 2t - 4D \sin 2t)</m></p>
<p><m> - (-2C \sin 2t + 2D \cos 2t) + C \cos 2t + D \sin 2t</m></p>
<p><m> = \sin 2t (10C + 5D) + \cos 2t (-10D + 5C) = 25 \cos 2t</m></p>
<p><m> \implies 10C + 5D = 0, -10D + 5C = 25 \implies C = 1, D = -2.</m></p>
<p>So <m>Y_3 = \cos 2t - 2 \sin 2t.</m></p>

<p>Let <m>Y_4</m> be a solution of <m>y''' - y'' - y' + y = t^2.</m></p>
<p>First ansatz <m>Y_4 = Et^2 + Ft + G.</m></p>
<p>Exp. Coeff. = <alert>0</alert>, not a root. <m>Y'_4 = 2Et + F, Y''_4 = 2E, Y'''_4 = 0.</m></p>
<p><m>Y'''_4 - Y''_4 - Y'_4 + Y_4 = 0 - 2E - (2Et + F) + Et^2 + Ft + G</m></p>
<p><m> = Et^2 + (F - 2E)t + G - 2E - F</m></p>
<p><m> \implies E = 1, F - 2E = 0, G - 2E - F = 0</m></p>
<p><m> \implies E = 1, F = 2, G = 4.</m></p>
<p>So <m>Y_4 = t^2 + 2t + 4.</m></p>

<p>By the principle of superposition,</p>
<p><m>Y = Y_1 + Y_2 + Y_3 + Y_4</m></p>
<p><m> = 2t^2 e^t + te^{-t} + \cos 2t - 2 \sin 2t + t^2 + 2t + 4</m></p>
<p>is a particular solution. The general solution is then</p>
<p><m>y = y_c + Y</m></p>
<p><m> = C_1 e^{-t} + C_2 e^t + C_3 t e^t + 2t^2 e^t + te^{-t} + \cos 2t - 2 \sin 2t + t^2 + 2t + 4.</m></p>


</section>