<?xml version="1.0" encoding="UTF-8"?>

<section xml:id="sec-1st-order-linear" xmlns:xi="http://www.w3.org/2001/XInclude">
  <title>First-order Linear ODEs</title>
<theorem xml:id="thm-1st-order-linear">
  <p>Consider a first-order linear ODE in its <alert>standard form</alert> <me>y' + p(t)y = g(t).</me></p>
  <p>We solve it by first calculating the <alert>integrating factor</alert> <me>\mu(t) = e^{\int p(t)dt},</me></p>
  <p>then the formula of the <alert>general solution</alert> is <me>y(t) = \frac{\int \mu(t)g(t)dt}{\mu(t)}.</me></p>
</theorem>

<proof>
  <p>How comes the formula? Observe that <me>e^{\int p(t)dt}(y' + p(t)y) = \left(e^{\int p(t)dt}y\right)'.</me></p>
  <p>In general, any function <m>\mu(t)</m> making <me>\mu(t)(y'(t) + p(t)y(t)) = (\mu(t)y(t))'</me> is called an integrating factor. To satisfy this equation, we calculate that</p>
  <me>RHS = \mu'(t)y(t) + \mu(t)y'(t)</me>
  <p>So <m>LHS = RHS</m> means</p>
  <md>
  <mrow>\amp \mu(t)y'(t) + \mu(t)p(t)y(t) = \mu'(t)y(t) + \mu(t)y'(t)</mrow>
  <mrow>\implies \amp \mu(t)p(t)y(t) = \mu'(t)y(t) \Rightarrow \mu'(t) = \mu(t)p(t)</mrow>
  <mrow>\implies \amp \frac{\mu'(t)}{\mu(t)} = p(t) \Rightarrow \ln|\mu(t)| = \int p(t)dt</mrow>
  <mrow>\implies \amp \mu(t) = e^{\int p(t)dt}.</mrow>
  </md>

  <p>Now that we found the <m>\mu(t)</m>, Recall that the ODE we intend to solve is</p>
  <md>
  <mrow> \amp y'(t) + p(t)y(t) = g(t)</mrow>
  <mrow>\implies \amp \mu(t)(y'(t) + p(t)y(t)) = \mu(t)g(t).</mrow>
  </md>
  <p>Thus, we conclude that</p>
  <me>(\mu(t)y(t))' = \mu(t)g(t).</me>
<p>Integrate both sides:</p>
<md>
<mrow>\amp \mu(t)y(t) = \int \mu(t)g(t)dt</mrow>
<mrow>\implies \amp y(t) = \frac{\int \mu(t)g(t)dt}{\mu(t)}.</mrow>
</md>
</proof>

<remark>
<ul>
  <li>This formula <alert>ONLY</alert> works for the <alert>standard form</alert>. Before using it, get the standard form first.</li>
  <li>When integrating <m>p(t)</m>, no need to worry about the constant or the absolute value. They make no difference.</li>
  <li>The arbitrary constant in the general solution appears as <alert>a part</alert> of the numerator, not outside of the fraction. It might be helpful to write the formula of the general solution as 
  <me>y(t) = \frac{\int \mu(t)g(t)dt + C}{\mu(t)}.</me>
  From this formula, it is clear that <m>C</m> is a pure constant only when <m>\mu(t)</m> is a constant. This case is very rare, and only happens when <m>p(t)=0</m>. </li>
</ul>
</remark>

<example>
  <title>Solve <m>y' + 2y = e^{3t}, \quad y(0) = 3.</m></title>
  <p><ul>
    <li>Already in standard form.</li>
    <li>Integrating factor: <m>\mu(t) = e^{\int 2dt} = e^{2t}.</m></li>
    <li>General solution:
    <md>
    <mrow>\amp y(t) = \frac{\int e^{2t}e^{3t}dt}{e^{2t}} = \frac{\int e^{5t}dt}{e^{2t}} = e^{-2t}\left(\frac{1}{5}e^{5t} + C\right).</mrow>
    <mrow>\implies \amp y(t) = \frac{1}{5}e^{3t} + Ce^{-2t}.</mrow>
    </md>
    </li>
  </ul></p>
  <p>Digression: What if we keep the constant in the integrating factor?</p>
<ul>
  <li>Integrating factor: <m>\mu(t) = e^{\int 2dt + D} = e^{2t + D} = e^{2t} e^{D}.</m></li>
  <li><p>General solution:
  <md>
    <mrow>y(t) \amp = \frac{\int e^{2t} e^{3t} e^{D} dt}{e^{2t} e^{D}} = 
    \frac{\int e^{5t} \cancel{e^D} dt}{e^{2t} \cancel{e^D}} = \frac{\frac{1}{5} e^{5t} + C}{e^{2t}}</mrow>
    <mrow>\amp = \frac{1}{5} e^{3t} + C e^{-2t}.</mrow>
  </md>
  So the extra constant in the integrating factor does not make any difference!</p>
</li>
</ul>
  <p> Coming back to the problem, we have obtained the general solution. But we are not done yet. We are given an IVP, so we need to take care of the initial condition.</p>
<ul>
  <li>Determine <m>C</m> by the initial condition:
  <me>y(0) = 3 \Rightarrow \frac{1}{5} + C = 3 \Rightarrow C = \frac{14}{5}.</me>
  </li>
</ul>
<p> <alert>Conclusion:</alert> The solution of the IVP is
  <me>y(t) = \frac{1}{5} e^{3t} + \frac{14}{5} e^{-2t}</me  >
</p>
</example>

<example>
  <title>Solve <m>ty' - y = t^3, \quad y(1) = 0.</m></title>
  <statement>
  <ul>
    <li>Standard form: <m>y' - \frac{1}{t}y = t^2.</m></li>
  <li><p>Integrating factor: <m>\mu(t) = e^{-\int \frac{1}{t} dt} = e^{-\ln |t|} = \frac{1}{t}.</m></p>
  <p><alert>Warning! Saying <m>e^{-\ln t} = -t</m> commits the crime of abusing algebra, which is punishable by banishment to the STEM. </alert></p></li>
  <li>General solution:
  <md>
  <mrow>y(t) \amp = \frac{\int \frac{1}{t} \cdot t^2 dt + C}{\frac{1}{t}} = t \left( \int dt + C \right)</mrow>
  <mrow>\amp = t \left( \frac{1}{2}t^2 + C \right) = \frac{1}{2}t^3 + Ct.</mrow>
  </md></li>
  <li>Determine <m>C</m> by initial value:
  <me>y(1) = 0 \Rightarrow \frac{1}{2} + C = 0 \Rightarrow C = -\frac{1}{2}.</me></li>
  <li>Solution of the IVP:
  <me>y(t) = \frac{1}{2}t^3 - \frac{1}{2}t.</me></li>
</ul>
</statement>
</example>

<example>
  <title>Solve <m>(\sin t) y' + (\cos t) y = \sin^2 t, \quad 0 \lt t \lt \pi.</m></title>
  <statement>
  <ul>
    <li>Standard form: <m>y' + \frac{\cos t}{\sin t} y = \sin t.</m></li>
    <li><p>Integrating factor: <m>\mu(t) = e^{\int \frac{\cos t}{\sin t} dt}</m></p>
  <md>
  <mrow>\int \frac{\cos t}{\sin t} dt = \int \frac{d(\sin t)}{\sin t} = \ln |\sin t|.</mrow>
  <mrow>\implies \mu(t) = e^{\ln |\sin t|} = \sin t.</mrow>
  </md>
  <p>Note that <m>0 \lt t \lt \pi\Rightarrow \sin t \gt 0, | \sin t | = \sin t.</m></p></li>
    <li><p>General solution: <m>y(t)  = \dfrac{\int \sin^2 t \, dt + C}{\sin t}</m></p>
    <p>We calculate the integral in the numerator:
    <md>
    <mrow>\int \sin^2 t \, dt \amp = \int \frac{1 - \cos 2t}{2} \, dt = \frac{1}{2} \int (1 - \cos 2t) \, dt</mrow>
    <mrow>\amp = \frac{1}{2} t - \frac{1}{4} \sin 2t + C.</mrow>
    </md></p>
    <p>Thus the general solution is of the form
    <md>
    <mrow>y(t) \amp = \frac{\frac{1}{2}t - \frac{1}{4}\sin 2t + C}{\sin t} = \frac{t}{2\sin t} - \frac{\sin 2t}{4\sin t} + \frac{C}{\sin t}</mrow>
    <mrow>\amp = \frac{t}{2\sin t} - \frac{\cos t}{2} + \frac{C}{\sin t},</mrow>
    </md>
    where in the last step we used the identity <m>\sin 2t = 2 \sin t \cos t</m>.</p>
    </li>
  </ul>
</statement>
</example>

<example>
  <title>Solve <m>ty' + 2y = t(\ln 3t)^2.</m></title>
  <statement>
  <ul>
    <li>Standard form: <m>y' + \frac{2}{t}y = (\ln 3t)^2.</m></li>
  <li>Integrating factor: <m>\mu(t) = e^{\int \frac{2}{t}dt} = e^{2 \ln t} = t^2.</m></li>
  <li><p>General solution: <me>y(t) = \frac{\int t^2(\ln 3t)^2dt + C}{t^2}.</me></p>
  <p> We calculate the integral in the numerator:
  <md><mrow>\int t^2(\ln 3t)^2 dt \amp = \frac{1}{3}t^3(\ln 3t)^2 - \int \frac{1}{3}t^3 \cdot 2\ln 3t \cdot \frac{1}{3} \cdot 3 dt</mrow>
  <mrow>\amp = \frac{1}{3}t^3(\ln 3t)^2 - \frac{2}{3}\int t^2 \ln 3t \, dt</mrow>
  <mrow>\amp= \frac{1}{3}t^3(\ln 3t)^2 - \frac{2}{3}\left(\frac{1}{3}t^3 \ln 3t - \int \frac{1}{3}t^3 \cdot \frac{1}{3t} \cdot 3 dt\right)</mrow>
  <mrow>\amp= \frac{1}{3}t^3(\ln 3t)^2 - \frac{2}{9}t^3 \ln 3t + \frac{2}{9} \cdot \frac{1}{3}t^3 + C</mrow>
  <mrow>\amp= \frac{1}{3}t^3(\ln 3t)^2 - \frac{2}{9}t^3 \ln 3t + \frac{2}{27}t^3 + C</mrow>
  </md>
  </p>
  <p> So we conclude the general solution as
  <md>
  <mrow>y(t) \amp = \frac{\frac{1}{3}t^3(\ln 3t)^2 - \frac{2}{9}t^3 \ln 3t + \frac{2}{27}t^3 + C}{t^2}</mrow>
  <mrow>\amp = \frac{1}{3}t(\ln 3t)^2 - \frac{2}{9}t \ln 3t + \frac{2}{27}t + \frac{C}{t^2}</mrow>
  </md>
  </p>
  </li>
</ul>
</statement>
</example>

<example>
  <title>Solve <m>y' + y = \cos 2t.</m></title>
  <statement>
  <ul>
    <li>Already in standard form.</li>
    <li>Integrating factor: <m>\mu(t) = e^{\int dt} = e^t.</m></li>
    <li><p>General solution:
    <md><mrow>y(t) \amp = \dfrac{\int e^t \cos 2t \, dt }{e^{t}} </mrow>
    <mrow>\amp =\cdots = \frac{1}{5}e^t \cos 2t + \frac{2}{5}e^t \sin 2t + C e^{-t}</mrow>
    </md>
    </p> 
    <p>How to calculate the integral?
    <md>
    <mrow>\int e^t \cos 2t \, dt \amp = e^t \cos 2t - \int e^t (-2 \sin 2t) \, dt</mrow>
    <mrow>\amp = e^t \cos 2t + 2 \int e^t \sin 2t \, dt</mrow>
    <mrow>\amp = e^t \cos 2t + 2\left(e^t \sin 2t - \int e^t (2 \cos 2t) \, dt\right)</mrow>
    <mrow>\amp = e^t \cos 2t + 2e^t \sin 2t - 4 \int e^t \cos 2t \, dt</mrow>
    </md></p>
    <p>So we have
    <md>
    <mrow>\amp 5 \int e^t \cos 2t \, dt = e^t \cos 2t + 2e^t \sin 2t+C</mrow>
    <mrow>\implies \amp  \int e^t \cos 2t \, dt = \frac{1}{5} e^t \cos 2t + \frac{2}{5} e^t \sin 2t+C</mrow>
    </md>
    </p>
    <p>Then we conclude the general solution as
    <md>
    <mrow>y(t) \amp =\dfrac{\frac{1}{5} e^t \cos 2t + \frac{2}{5} e^t \sin 2t+C }{e^{t}}</mrow>
    <mrow>\amp = \frac{1}{5} e^t \cos 2t + \frac{2}{5} e^t \sin 2t + C e^{-t}</mrow>
    </md>
    </p>
    </li>
  </ul>
</statement>
</example>

<example>
  <title>Solve <m>y' - (\tan t)y = \sec^2 t.</m></title>
  <statement>
  <ul>
    <li>Already in standard form.</li>
  <li><p>Integrating factor: <m>\mu(t) = e^{-\int \tan t \, dt} = e^{\ln |\cos t|} = \cos t.</m></p>
  <p>Here we ignored the absolute value (why can we do that?).</p></li>
  <li><p>General solution:
  <md>
  <mrow> y(t) \amp = \frac{\int \cos t \cdot \sec^2 t \, dt + C}{\cos t} = \frac{\int \sec t \, dt + C}{\cos t}</mrow>
  <mrow>\amp = \frac{\ln |\sec t + \tan t| + C}{\cos t}</mrow>
  </md></p>
  <p>Please make sure you know how to integrate <m>\sec t</m>.</p>
  </li>
  </ul>
  </statement>
</example>

<example xml:id="ex-1st-order-linear-piecewise"> 
  <title>Solve <me>y' + y = g(t), \, y(0) = 0, \, g(t) = \begin{cases} 1 \amp 0 \leq t \leq 1 \\ 0 \amp t \gt 1 \end{cases}</me>. Find the solution of the IVP that is continuous everywhere</title>
  <statement>
  <p>General principle: Solve the ODE on each individual interval. Determine the constants by either the initial condition or continuity at the boundary .</p>
  <p>On the interval <m>[0,1], \, y' + y = 1.</m></p>
  <ul>
    <li>Integrating factor: <m>\mu(t) = e^{\int dt} = e^t.</m></li>
    <li>General solution:
    <me>y(t) = \frac{\int e^t \cdot 1 \, dt + C}{e^t} = \frac{e^t + C}{e^t} = 1 + Ce^{-t}.</me>
    </li>
    <li>Initial condition <m>y(0) = 0 \Rightarrow 1 + Ce^0 = 0 \Rightarrow C = -1.</m></li>
    <li>We conclude that on <m>[0,1], \, y(t) = 1 - e^{-t}.</m></li>
  </ul>
  <p>On the interval <m>(1, \infty), \, y' + y = 0.</m></p>
  <ul>
    <li>Integrating factor: <m>\mu(t) = e^{\int dt} = e^t.</m></li>
    <li>General solution:
    <me>y(t) = \frac{\int e^t \cdot 0 \, dt + C}{e^t} = \frac{C}{e^t} = Ce^{-t}.</me></li>
    <li>On <m>(1, \infty), \, y(t) = Ce^{-t}.</m></li>
  </ul>
  <p>So the solution of the IVP is
  <me>y(t) = \begin{cases} 1 - e^{-t} \amp t \in [0,1] \\ Ce^{-t} \amp t \in (1,\infty) \end{cases}</me></p>
  <p>To make sure <m>y(t)</m> is continuous, we need <m>\lim_{t \to 1^-} y(t) = \lim_{t \to 1^+} y(t).</m>. This is to say <m>1 - e^{-1} = Ce^{-1} \Rightarrow C = (e - 1).</m></p>
  <p>Conclusion: the continuous solution of the IVP is
  <me>y(t) = \begin{cases} 1 - e^{-t} \amp t \in [0,1] \\ (e - 1)e^{-t} \amp t \in (1,\infty) \end{cases}</me></p>
</statement>
</example>

</section>
