<?xml version="1.0" encoding="UTF-8"?>

<section xml:id="sec-laplace-transform" xmlns:xi="http://www.w3.org/2001/XInclude">
  <title>Laplace Transform and Examples</title>

<subsection>
<title>Integral Transform</title>

<definition>
<p>Let <m>K(s, t)</m> be a function with two real variables. Given a function <m>f(t)</m> defined on a set <m>D</m>, the following integral
<me>F(s) = \int_D K(s, t)f(t)dt</me>
defines a new function <m>F(s)</m>. The map sending <m>f(t)</m> to <m>F(s)</m> is called an <term>integral transform</term>. The function <m>K(s, t)</m> is called the <term>kernel</term> of the integral transform.</p>
</definition>

<remark>
<p>Note that when <m>D</m> is an <alert>infinite</alert> interval, the integral defining <m>F(s)</m> is improper and might not converge for all real numbers <m>s</m>. In this case, the domain of new function <m>F(s)</m>, i.e., the set of <m>s</m> such that the integral converges, is not expected to be <m>(-\infty, \infty).</m></p>
</remark>

<p>Integral transforms appears in many discussions of mathematics, physics, engineering, and computer science. The most important one is the <term>Fourier transform</term>, where
<me>D = (-\infty, \infty), K(s, t) = e^{-ist}.</me>
In other words, Fourier transform sends <m>f(t)</m> to a <alert>complex function</alert>
<me>F(s) = \int_{-\infty}^{\infty} f(t)e^{-ist} dt</me>
Note that when <m>D</m> is an <alert>infinite</alert> interval, the integral defining <m>F(s)</m> is improper and might not converge for all real numbers <m>s</m>. In this case, the domain of new function <m>F(s)</m>, i.e., the set of <m>s</m> such that the integral converges, is not expected to be <m>(-\infty, \infty).</m></p>

<p>Fourier transform is widely used, including but not limited to, partial differential equations, computer graphics, machine learning, etc. We will not require it in this course because it is necessary to know complex function. </p>

<p>In this course, we mainly focus on the <alert>Laplace transform</alert>. </p>

<definition> 
<p>The <term>Laplace transform</term> is the integral transform with
<me>D = [0, \infty), K(s, t) = e^{-st}.</me>
In other words, Laplace transform sends
<me>f(t) \mapsto F(s) = \int_{0}^{\infty} f(t)e^{-st} dt</me>
The function <m>F(s)</m> is often denoted by <m>\mathcal{L}\{f(t)\}.</m></p>
<p>The domain of <m>F(s)</m> depends on <m>f(t)</m>, determined by the convergence of the improper integral, i.e.,
<me>\lim_{b \to \infty} \int_{0}^{b} f(t)e^{-st} dt</me> should exist.</p>
</definition>
</subsection>

<subsection>
<title>Examples of Laplace transforms</title>

<example>
<title>Evaluate <m>\mathcal{L}\{1\}</m></title>
<p><md>
<mrow>\mathcal{L}\{1\} = \ \amp \int_{0}^{\infty} e^{-st} dt = \left. \dfrac{e^{-st}}{-s} \right|_{0}^{\infty} </mrow>
<mrow> = \ \amp \left( \lim_{t \to \infty} \dfrac{e^{-st}}{-s} \right) - \frac{1}{-s}.</mrow>
</md></p>
<ul>
<li>If <m>s \gt 0</m>, then <m>\lim_{t \to \infty} \dfrac{e^{-st}}{-s} = 0.</m> The integral converges. In this case, <me>F(s) = 0 - \frac{1}{-s} = \dfrac{1}{s}.</me></li>
<li>If <m>s \lt 0</m>, then <m>\lim_{t \to \infty} \dfrac{e^{-st}}{-s} = +\infty.</m> The integral diverges.</li>
<li>If <m>s = 0</m>, we cannot use the previous formula because <m>1/s</m> makes no sense. But looking back to the integral, note that when <m>s = 0, e^{-st} = 1.</m> In this case, <me>\int_{0}^{\infty} e^{-st} dt = \int_{0}^{\infty} 1 dt</me> also diverges.</li>
</ul>
<p>Conclusion: <me>\mathcal{L}\{1\} = \dfrac{1}{s}, \quad s \gt 0.</me></p>
</example>

<example>
<title>Evaluate <m>\mathcal{L}\{t\}</m></title>
<p><md>
<mrow>\mathcal{L}\{t\} = \ \amp  \int_{0}^{\infty} te^{-st} dt = -\dfrac{1}{s} te^{-st} \bigg|_{0}^{\infty} - \int_{0}^{\infty} 1 \cdot \left(-\dfrac{1}{s} e^{-st}\right) dt</mrow>
<mrow> = \ \amp  -\dfrac{1}{s} \left( \lim_{t \to \infty} te^{-st} - 0 \right) + \dfrac{1}{s} \int_{0}^{\infty} e^{-st} dt</mrow>
</md>
We have seen that <m>\int_{0}^{\infty} e^{-st} dt</m> converges if and only if <m>s \gt 0.</m> In this case, using L'HÃ´pital's rule, 
<me>\lim_{t \to \infty} te^{-st} = \lim_{t \to \infty} \dfrac{t}{e^{st}} = 0. </me>
so 
<md>
<mrow>\mathcal{L}\{t\} = \ \amp \int_{0}^{\infty} te^{-st} dt = -\dfrac{1}{s} te^{-st} \bigg|_{0}^{\infty} - \int_{0}^{\infty} 1 \cdot \left(-\dfrac{1}{s} e^{-st}\right) dt</mrow>
<mrow> = \ \amp -\dfrac{1}{s} \left( \lim_{t \to \infty} te^{-st} - 0 \right) + \dfrac{1}{s} \int_{0}^{\infty} e^{-st} dt</mrow>
<mrow> = \ \amp -\dfrac{1}{s} \cdot (0 - 0) + \dfrac{1}{s} \cdot \dfrac{1}{s} = \dfrac{1}{s^2}.</mrow>
</md></p>
<p>Conclusion:
<me>\mathcal{L}\{t\} = \dfrac{1}{s^2}, \quad s \gt 0.</me></p>
</example>

<example>
<title>Evaluate <m>\mathcal{L}\{t^n\}</m></title>
<p><md>
<mrow>\mathcal{L}\{t^n\} = \ \amp \int_{0}^{\infty} t^n e^{-st} dt</mrow>
<mrow> = \ \amp -\dfrac{1}{s} t^n e^{-st} \bigg|_{0}^{\infty} - \int_{0}^{\infty} nt^{n-1} \left(-\dfrac{1}{s} e^{-st}\right) dt</mrow>
<mrow> = \ \amp -\dfrac{1}{s} \left( \lim_{t \to \infty} t^n e^{-st} - 0 \right) + \dfrac{n}{s} \int_{0}^{\infty} t^{n-1} e^{-st} dt</mrow>
</md>
Clearly, <m>\lim_{t \to \infty} t^n e^{-st}</m> exists if and only if <m>s \gt 0</m>, and the limit is 0. So we have obtained that for <m>s \gt 0,</m>
<me>\mathcal{L}\{t^n\} = -\frac{n}{s} \int_{0}^{\infty} t^{n-1} e^{-st} dt = -\frac{n}{s} \mathcal{L}\{t^{n-1}\}.</me>
This defines a recursion of <m>\mathcal{L}\{t^n\}</m> that can be easily solved:
<md>
<mrow>\mathcal{L}\{t^n\} = \ \amp \dfrac{n}{s} \mathcal{L}\{t^{n-1}\} = \dfrac{n}{s} \cdot \dfrac{n - 1}{s} \mathcal{L}\{t^{n-2}\}</mrow>
<mrow> = \ \amp \cdots = \dfrac{n}{s} \cdot \dfrac{n - 1}{s} \cdots \dfrac{2}{s} \cdot \dfrac{1}{s} \mathcal{L}\{1\}</mrow>
<mrow> = \ \amp \dfrac{n \cdot (n - 1) \cdots 2 \cdot 1}{s^{n + 1}} = \dfrac{n!}{s^{n + 1}}.</mrow>
</md></p>
<p>Conclusion:
<me>\mathcal{L}\{t^n\} = \dfrac{n!}{s^{n + 1}}, \quad s \gt 0.</me>
For example,
<me>\mathcal{L}\{t^2\} = \dfrac{2!}{s^3}, \quad \mathcal{L}\{t^3\} = \dfrac{3!}{s^4}, \quad \mathcal{L}\{t^4\} = \dfrac{4!}{s^5}, \quad s \gt 0.</me>
Note that the power of <m>s</m> in the denominator is 1 larger than the power of <m>t.</m></p>
</example>

<example>
<title>Evaluate <m>\mathcal{L}\{e^{-3t}\}</m> and <m>\mathcal{L}\{e^{5t}\}</m></title>
<ul>
<li>By definition,
<md>
<mrow>\mathcal{L}\{e^{-3t}\} = \ \amp \int_{0}^{\infty} e^{-3t} e^{-st} dt = \int_{0}^{\infty} e^{-(s + 3)t} dt</mrow>
<mrow> = \ \amp \frac{1}{-(s + 3)} e^{-(s + 3)t} \bigg|_{0}^{\infty} = \frac{1}{-(s + 3)} \left( \lim_{t \to \infty} e^{-(s + 3)t} - 1 \right)</mrow>
</md>
Clearly, <m>\lim_{t \to \infty} e^{-(s + 3)t}</m> exists when <m>s + 3 \gt 0,</m> i.e., <m>s \gt -3.</m> The limit is zero. So
<me>\mathcal{L}\{e^{-3t}\} = \frac{1}{-(s + 3)} (0 - 1) = \frac{1}{s + 5}, \quad s \gt -3.</me></li>
<li>By definition,
<md>
<mrow>\mathcal{L}\{e^{5t}\} = \ \amp \int_{0}^{\infty} e^{5t} e^{-st} dt = \int_{0}^{\infty} e^{-(s - 5)t} dt</mrow>
<mrow> = \ \amp \frac{1}{-(s - 5)} e^{-(s - 5)t} \bigg|_{0}^{\infty} = \frac{1}{-(s - 5)} \left( \lim_{t \to \infty} e^{-(s - 5)t} - 1 \right)</mrow>
</md>
Clearly, <m>\lim_{t \to \infty} e^{-(s - 5)t}</m> exists when <m>s - 5 \gt 0,</m> i.e., <m>s \gt 5.</m> The limit is zero. So
<me>\mathcal{L}\{e^{5t}\} = \frac{1}{-(s - 5)} (0 - 1) = \frac{1}{s - 5}, \quad s \gt 5.</me></li>
</ul>
</example>

<example>
<title>Evaluate <m>\mathcal{L}\{e^{at}\}</m></title>
<p>By definition,
<md>
<mrow>\mathcal{L}\{e^{at}\} = \ \amp \int_{0}^{\infty} e^{at} e^{-st} dt = \int_{0}^{\infty} e^{-(s - \alpha)t} dt</mrow>
<mrow> = \ \amp \frac{1}{-(s - \alpha)} e^{-(s - \alpha)t} \bigg|_{0}^{\infty} = \frac{1}{-(s - \alpha)} \left( \lim_{t \to \infty} e^{-(s - \alpha)t} - 1 \right)</mrow>
</md>
Clearly, <m>\lim_{t \to \infty} e^{-(s - \alpha)t}</m> exists when <m>s - \alpha \gt 0,</m> i.e., <m>s \gt \alpha.</m> The limit is zero. So
<me>\mathcal{L}\{e^{at}\} = \frac{1}{s - \alpha}, \quad s \gt \alpha.</me></p>
</example>
<example>
<title>Evaluate <m>\mathcal{L}\{\sin 2t\}</m></title>
<p><md>
<mrow>\mathcal{L}\{\sin 2t\} = \ \amp \int_{0}^{\infty} \sin 2t \, e^{-st} dt</mrow>
<mrow> = \ \amp -\dfrac{1}{s} \sin 2t \, e^{-st} \bigg|_{0}^{\infty} - \int_{0}^{\infty} 2 \cos 2t \left(-\dfrac{1}{s} e^{-st}\right) dt</mrow>
<mrow> = \ \amp -\dfrac{1}{s} \left( \lim_{t \to \infty} e^{-st} \sin 2t - 0 \right) + \frac{2}{s} \int_{0}^{\infty} \cos 2t \, e^{-st} dt</mrow>
</md>
Clearly, <m>\lim_{t \to \infty} e^{-st} \sin 2t</m> exists <alert>iff</alert> <m>s \gt 0,</m> and equals 0. So
<md>
<mrow>\mathcal{L}\{\sin 2t\} =\ \amp -\frac{2}{s} \int_{0}^{\infty} \cos 2t \, e^{-st} dt</mrow>
<mrow> = \ \amp \frac{2}{s} \left( -\dfrac{1}{s} \cos 2t \, e^{-st} \bigg|_{0}^{\infty} - \int_{0}^{\infty} (-2 \sin 2t) \left(-\dfrac{1}{s} e^{-st}\right) dt \right)</mrow>
<mrow> = \ \amp -\frac{2}{s^2} \left( \lim_{t \to \infty} \cos 2t \, e^{-st} - \cos 0 \, e^0 \right) - \frac{4}{s^2} \int_{0}^{\infty} \sin 2t \, e^{-st} dt</mrow>
</md>
Clearly when <m>s \gt 0,</m> <m>\lim_{t \to \infty} e^{-st} \cos 2t = 0.</m> So
<md>
<mrow>\mathcal{L}\{\sin 2t\} = \ \amp -\frac{2}{s^2} (0 - 1) - \frac{4}{s^2} \int_{0}^{\infty} \sin 2t \, e^{-st} dt</mrow>
<mrow> = \ \amp \frac{2}{s^2} - \frac{4}{s^2} \mathcal{L}\{\sin 2t\} \Rightarrow \left( 1 + \frac{4}{s^2} \right) \mathcal{L}\{\sin 2t\} = \frac{2}{s^2}</mrow>
</md>
So we conclude that
<me>\mathcal{L}\{\sin 2t\} = \frac{2}{s^2 + 4}, \quad s \gt 0.</me></p>
</example>

<example>
<title>Evaluate <m>\mathcal{L}\{\sin \beta t\}</m></title>
<p>With a similar procedure, we see that
<md>
<mrow>\mathcal{L}\{\sin \beta t\} = \ \amp \frac{\beta}{s^2} - \frac{\beta^2}{s^2} \mathcal{L}\{\sin \beta t\} \Rightarrow \left( 1 + \frac{\beta^2}{s^2} \right) \mathcal{L}\{\sin \beta t\} = \frac{\beta}{s^2}</mrow>
</md>
So we conclude that
<me>\mathcal{L}\{\sin \beta t\} = \frac{\beta}{s^2 + \beta^2}, \quad s \gt 0.</me></p>
</example>

<example>
<title>Evaluate <m>\mathcal{L}\{\cos \beta t\}</m></title>
<p>With a similar procedure, we see that
<md>
<mrow>\mathcal{L}\{\cos \beta t\} = \ \amp \frac{1}{s} - \frac{\beta^2}{s^2} \mathcal{L}\{\cos \beta t\} \Rightarrow \left( 1 + \frac{\beta^2}{s^2} \right) \mathcal{L}\{\cos \beta t\} = \frac{s}{s^2}</mrow>
</md>
So we conclude that
<me>\mathcal{L}\{\cos \beta t\} = \frac{s}{s^2 + \beta^2}, \quad s \gt 0.</me></p>
</example>

<theorem>
<title>Linearity of Laplace transform</title>
<p>For every real numbers <m>\alpha, \beta,</m>
<me>\mathcal{L}\{\alpha f(t) + \beta g(t)\} = \alpha \mathcal{L}\{f(t)\} + \beta \mathcal{L}\{g(t)\}.</me></p>
</theorem>

<proof> 
<p> It follows from the linearity of integrals.
<md>
<mrow>\mathcal{L}\{\alpha f(t) + \beta g(t)\} = \ \amp \int_{0}^{\infty} (\alpha f(t) + \beta g(t)) e^{-st} dt</mrow>
<mrow> = \ \amp \alpha \int_{0}^{\infty} f(t)e^{-st} dt + \beta \int_{0}^{\infty} g(t)e^{-st} dt</mrow>
<mrow> = \ \amp \alpha \mathcal{L}\{f(t)\} + \beta \mathcal{L}\{g(t)\}.</mrow>
</md></p>
</proof>

<definition>
<title>Hyperbolic functions</title>
<p>Recall that from the Eulerâs formula, the usual sine and cosine functions may also be expressed as
<me>\sin t = \frac{e^{it} - e^{-it}}{2i}, \quad \cos t = \frac{e^{it} + e^{-it}}{2}.</me></p>
<p>The <term>hyperbolic functions</term> are defined similarly:
<me>\sinh t = \frac{e^t - e^{-t}}{2}, \quad \cosh t = \frac{e^t + e^{-t}}{2}.</me></p>
<p>These functions are widely used in engineering practices.</p>
</definition>

<p>The Laplace transform of hyperbolic functions can be obtained via linearity. For every <m>k \gt 0:</m>
<md>
<mrow>\mathcal{L}\{\sinh kt\} = \ \amp \mathcal{L}\left\{ \frac{e^{kt} - e^{-kt}}{2} \right\} = \frac{1}{2} \mathcal{L}\{e^{kt}\} - \frac{1}{2} \mathcal{L}\{e^{-kt}\}</mrow>
<mrow> = \ \amp \frac{1}{2} \cdot \frac{1}{s - k} - \frac{1}{2} \cdot \frac{1}{s + k} = \frac{1}{2} \cdot \frac{s + k - (s - k)}{(s - k)(s + k)} = \frac{k}{s^2 - k^2}.</mrow>
</md>
<md>
<mrow>\mathcal{L}\{\cosh kt\} = \ \amp \mathcal{L}\left\{ \frac{e^{kt} + e^{-kt}}{2} \right\} = \frac{1}{2} \mathcal{L}\{e^{kt}\} + \frac{1}{2} \mathcal{L}\{e^{-kt}\}</mrow>
<mrow> = \ \amp \frac{1}{2} \cdot \frac{1}{s - k} + \frac{1}{2} \cdot \frac{1}{s + k} = \frac{1}{2} \cdot \frac{s + k + (s - k)}{(s - k)(s + k)} = \frac{s}{s^2 - k^2}.</mrow>
</md>
</p>
</subsection>
<subsection>
<title>Summary of basic formulas for Laplace transform</title>

<ul>
<li>Power functions:
<me>\mathcal{L}\{1\} = \dfrac{1}{s}, \quad \mathcal{L}\{t\} = \frac{1}{s^2}, \quad \mathcal{L}\{t^n\} = \frac{n!}{s^{n + 1}}, \quad s \gt 0.</me>
Then by linearity, we may obtain the Laplace transform of all polynomial functions, e.g., <me>\mathcal{L}\{1 + 5t + 3t^2\} = \mathcal{L}\{1\} + 5\mathcal{L}\{t\} + 3\mathcal{L}\{t^2\} = \dfrac{1}{s} + \frac{5}{s^2} + 3 \cdot \frac{2!}{s^3} = \dfrac{1}{s} + \frac{5}{s^2} + \frac{6}{s^3}.</me></li>

<li>Exponential functions: for every real number <m>\alpha,</m>
<me>\mathcal{L}\{e^{\alpha t}\} = \frac{1}{s - \alpha}, \quad s \gt \alpha.</me></li>

<li>Trigonometric functions: for every <m>\beta \gt 0,</m>
<me>\mathcal{L}\{\cos \beta t\} = \frac{s}{s^2 + \beta^2}, \quad \mathcal{L}\{\sin \beta t\} = \frac{\beta}{s^2 + \beta^2}, \quad s \gt 0.</me></li>

<li>Hyperbolic functions, for every <m>k \gt 0,</m>
<me>\mathcal{L}\{\cosh kt\} = \frac{s}{s^2 - k^2}, \quad \mathcal{L}\{\sinh kt\} = \frac{k}{s^2 - k^2}, \quad s \gt k.</me></li>
</ul>

</subsection>

<subsection>
<title>Existence of <m>\mathcal{L}\{f(t)\}</m> and its long term behavior</title>

<p>Recall: A function is piecewise continuous on <m>[0, \infty),</m> if in any subinterval <m>[a, b],</m> the function is continuous everywhere except at finitely many removable or jump discontinuities.</p>

<definition>
<p>A function is said to be <term>of exponential order</term> if there exist constants <m>c, M \gt 0</m> and <m>T \gt 0,</m> such that <me>|f(t)| \leq Me^{ct} \text{ for all } t \gt T.</me>
In other words, <m>|f(t)|</m> does not grow faster than a constant multiple of a simple exponential function <m>e^{ct}.</m></p>
</definition>

<p>Polynomial functions, simple exponential function <m>e^{at},</m> cosine and sine functions are of exponential order.</p>

<p>The function <m>f(t) = e^{t^2}</m> is not of exponential order, since for every possible <m>c \gt 0,</m>
<me>\left| \frac{e^{t^2}}{e^{ct}} \right| = e^{t^2 - ct} = e^{t^2(t - c)} \to \infty</me>
So <m>e^{t^2}</m> grows faster than any multiple of <m>e^{ct}.</m></p>

<theorem>
<title>Sufficient conditions for existence of Laplace transform</title>
<p>If <m>f</m> is piecewise continuous on <m>[0, \infty)</m> and of exponential order, then <m>\mathcal{L}\{f(t)\}</m> exists for <m>s \gt c.</m></p>
</theorem>

<proof>
<p>Since <m>f</m> is of exponential order, there exist <m>c \gt 0, M \gt 0, T \gt 0,</m> such that whenever <m>t \gt T, |f(t)| \leq Me^{ct}.</m> Using the number <m>T,</m> we rewrite
<me>\mathcal{L}\{f(t)\} = \int_{0}^{T} e^{-st} f(t) dt + \int_{T}^{\infty} e^{-st} f(t) dt = I_1 + I_2</me>
Since <m>f</m> is piecewise continuous, <m>I_1</m> exists.</p>
<p>For <m>I_2,</m> we use the inequality <m>|f(t)| \leq Me^{ct}</m> to show that
<me>\int_{T}^{\infty} |e^{-st} f(t)| dt = \int_{T}^{\infty} e^{-st} |f(t)| dt \leq \int_{T}^{\infty} e^{-st} e^{ct} dt</me>
Right-hand side is precisely <m>\mathcal{L}\{e^{ct}\}</m> that exists when <m>s \gt c.</m> In other words, <m>I_2</m> converges absolutely when <m>s \gt c.</m></p>
</proof>

<remark>
<p> These two conditions are sufficient but not necessary. In other words, <m>\mathcal{L}\{f(t)\}</m> exists does not mean that <m>f(t)</m> should satisfy these two conditions. </p>
<p> For example, the function <m>t^{-\frac{1}{2}}</m> is not piecewise continuous. The function <m>2te^{t^2} \cos e^{t^2}</m> is not of exponential order. But it is not difficult to see that both <m>\mathcal{L}\{t^{-\frac{1}{2}}\}</m> and <m>\mathcal{L}\{2te^{t^2} \cos e^{t^2}\}</m> exist.</p>
</remark>

<theorem>
<title>Long term behavior of <m>\mathcal{L}\{f(t)\}</m></title>
<p>If <m>f</m> is piecewise continuous on <m>[0, \infty)</m> and of exponential order, then the function <m>F(s) = \mathcal{L}\{f(t)\}</m> satisfies <m>\lim_{s \to \infty} F(s) = 0.</m></p>
</theorem>

<proof>
<p>Take <m>c, M, T \gt 0</m> as in the previous proof. Since <m>f</m> is piecewise continuous on <m>[0, T],</m> <m>f(x)</m> is bounded. By adjusting <m>M,</m> we may assume that <m>|f(t)| \leq Me^{ct}</m> on <m>[0, \infty).</m> Then we estimate that
<me>0 \leq |F(s)| \leq \int_{0}^{\infty} e^{-st} |f(t)| dt \leq \int_{0}^{\infty} e^{-st} e^{ct} dt = \int_{0}^{\infty} e^{-(s - c)t} dt = \frac{1}{s - c} \to 0, \text{ as } s \to \infty.</me>
The conclusion then follows from the squeeze theorem.</p>
</proof>

</subsection>
</section>